Refactored atomics and hashtable.
Hashtable proofs in progress; linsearch program and proofs broken.

mailbox/hashtable1.c
@@ -1,19 +1,10 @@
-#include <stdlib.h>
-//#include "threads.h"
 #include "atomics.h"
-//#include <stdatomic.h>
 
-void *surely_malloc (size_t n) {
-  void *p = malloc(n);
-  if (!p) exit(1);
-  return p;
-}
+typedef struct entry { atomic_loc *key; atomic_loc *value; } entry;
 
-typedef struct entry { int key; lock_t *lkey; int value; lock_t *lvalue; } entry;
+#define ARRAY_SIZE 16384
 
-#define ARRAY_SIZE 32
-
-entry *m_entries[ARRAY_SIZE];
+entry m_entries[ARRAY_SIZE];
 
 int integer_hash(int i){
   return (unsigned int) i * (unsigned int) 654435761;
@@ -22,21 +13,22 @@ int integer_hash(int i){
 void set_item(int key, int value){
   for(int idx = integer_hash(key);; idx++){
     idx &= ARRAY_SIZE - 1;
-    entry *e = m_entries[idx];
-    int *i = &(e->key);
-    lock_t *l = e->lkey;
-    int probed_key = simulate_atomic_load(i, l);
+    atomic_loc *i = m_entries[idx].key;
+    int probed_key = load_SC(i);
     if(probed_key != key){
       //The entry was either free, or contains another key.
       if (probed_key != 0)
 	continue;
-      int prev_key = simulate_atomic_CAS(i, l, 0, key);
-      if((prev_key != 0) && (prev_key != key))
-	continue; //Another thread just stole the slot for a different key.
+      int result = CAS_SC(i, 0, key);
+      //This bit is a little different, since C11 doesn't have a CAS that returns the old value.
+      if(!result){
+	//CAS failed, so a key has been added. Is it the one we're looking for?
+	probed_key = load_SC(i);
+	if(probed_key != key) continue; //Another thread just stole the slot for a different key.
+      }
     }
-    i = &(e->value);
-    l = e->lvalue;
-    simulate_atomic_store(i, l, value);
+    i = m_entries[idx].value;
+    store_SC(i, value);
     return;
   }
 }
@@ -44,18 +36,16 @@ void set_item(int key, int value){
 int get_item(int key){
   for(int idx = integer_hash(key);; idx++){
     idx &= ARRAY_SIZE - 1;
-    entry *e = m_entries[idx];
-    int *i = &(e->key);
-    lock_t *l = e->lkey;
-    int probed_key = simulate_atomic_load(i, l);
+    atomic_loc *i = m_entries[idx].key;
+    int probed_key = load_SC(i);
     if(probed_key == key){
-      i = &(e->value);
-      l = e->lvalue;
-      return simulate_atomic_load(i, l);
+      i = m_entries[idx].value;
+      return load_SC(i);
     }
     if (probed_key == 0)
       return 0;
   }
 }
 
-      
+int main(void){
+}
