mailbox/real_atomics.c
@@ -1,0 +1,31 @@
+#include "atomics.h"
+#include <stdatomic.h>
+
+typedef struct atomic_loc { atomic_int ai; } atomic_loc;
+
+atomic_loc *make_atomic(int i){
+  atomic_loc *a = malloc(sizeof(atomic_loc));
+  atomic_init(&(a->ai), i);
+  return a;
+}
+
+void free_atomic(atomic_loc *tgt){
+  free(tgt);
+}
+
+int load_SC(atomic_loc *tgt){
+  return atomic_load(&(tgt->ai));
+}
+
+void store_SC(atomic_loc *tgt, int v){
+  atomic_store(&(tgt->ai), v);
+}
+
+//The C builtin only returns a boolean.
+int CAS_SC(atomic_loc *tgt, int c, int v){
+  return atomic_compare_exchange_strong(&(tgt->ai), &c, v);
+}
+
+int load_relaxed(atomic_loc *tgt){
+  return atomic_load_explicit(&(tgt->ai), memory_order_relaxed);
+}
