mailbox/verif_hashtable1.v
@@ -1,26 +1,15 @@
-Require Import mailbox.verif_atomics.
 Require Import progs.ghost.
+Require Import mailbox.verif_atomics.
 Require Import progs.conclib.
 Require Import floyd.library.
 Require Import floyd.sublist.
 Require Import mailbox.hashtable1.
+Require Import mailbox.hashtable.
 
 Set Bullet Behavior "Strict Subproofs".
 
 Instance CompSpecs : compspecs. make_compspecs prog. Defined.
 Definition Vprog : varspecs. mk_varspecs prog. Defined.
-
-Definition surely_malloc_spec :=
- DECLARE _surely_malloc
-   WITH n:Z
-   PRE [ _n OF tuint ]
-       PROP (0 <= n <= Int.max_unsigned)
-       LOCAL (temp _n (Vint (Int.repr n)))
-       SEP ()
-    POST [ tptr tvoid ] EX p:_,
-       PROP ()
-       LOCAL (temp ret_temp p)
-       SEP (malloc_token Tsh n p * memory_block Tsh n p).
 
 Definition integer_hash_spec :=
  DECLARE _integer_hash
@@ -34,525 +23,11 @@ Definition integer_hash_spec :=
 
 Definition tentry := Tstruct _entry noattr.
 
-Definition entry_hists entries hists := fold_right sepcon emp (map (fun i =>
-  let '(hp, e) := (Znth i hists ([], []), Znth i entries Vundef) in
-    ghost_hist (fst hp) (field_address tentry [StructField _key] e) *
-    ghost_hist (snd hp) (field_address tentry [StructField _value] e)) (upto 32)).
-
-(* Maps are represented as partial association lists, with entries with key 0 considered to be empty. *)
-Fixpoint index_of (m : list (Z * Z)) (k : Z) :=
-  match m with
-  | [] => None
-  | (k1, v1) :: rest => if eq_dec k1 k then Some 0
-                        else option_map Z.succ (index_of rest k)
-  end.
-
-Lemma index_of_spec : forall k m, match index_of m k with
-  | Some i => 0 <= i < Zlength m /\ fst (Znth i m (0, 0)) = k /\ Forall (fun x => fst x <> k) (sublist 0 i m)
-  | None => ~In k (map fst m) end.
+Instance hf1 : hash_fun := { size := 16384; hash i := (i * 654435761) mod 16384 }.
 Proof.
-  induction m; simpl; auto; intros.
-  destruct a.
-  rewrite Zlength_cons.
-  pose proof (Zlength_nonneg m).
-  destruct (eq_dec z k).
-  { split; [omega|].
-    rewrite sublist_nil; auto. }
-  destruct (index_of m k); simpl.
-  - destruct IHm as (? & ? & ?); unfold Z.succ.
-    rewrite Znth_cons_eq, Z.add_simpl_r.
-    if_tac; [omega|].
-    split; [omega|].
-    split; auto.
-    rewrite sublist_0_cons, Z.add_simpl_r by omega; constructor; auto.
-  - tauto.
-Qed.
-
-(* Abstract properties of hashtables (of length 32) *)
-Definition hash i := (i * 654435761) mod 32.
-
-Definition rebase (m : list (Z * Z)) i := rotate m (Zlength m - i) (Zlength m).
-
-Lemma rebase_0 : forall m i d, 0 <= i < Zlength m -> Znth 0 (rebase m i) d = Znth i m d.
-Proof.
-  intros; unfold rebase.
-  destruct (eq_dec (Zlength m) 0).
-  { apply Zlength_nil_inv in e; subst.
-    rewrite rotate_nil, !Znth_nil; auto. }
-  pose proof (Zlength_nonneg m).
-  rewrite Znth_rotate; try omega.
-  f_equal.
-  rewrite <- Z.mod_add with (b := 1) by auto.
-  replace (0 - (Zlength m - i) + 1 * Zlength m) with i by omega.
-  apply Zmod_small; auto.
-Qed.
-
-Definition well_chained (m : list (Z * Z)) := forall k i, index_of (rebase m (hash k)) k = Some i ->
-  Forall (fun x => fst x <> 0) (sublist 0 i (rebase m (hash k))).
-
-Definition wf_map (m : list (Z * Z)) := NoDup (map fst m).
-
-Definition indices i j := (map (fun x => (i + x) mod 32) (upto (Z.to_nat ((j - i) mod 32)))).
-
-Fixpoint index_of' (m : list (Z * Z)) k :=
-  match m with
-  | [] => None
-  | (k1, v1) :: rest => if eq_dec k1 0 then Some 0 else
-                        if eq_dec k1 k then Some 0
-                        else option_map Z.succ (index_of' rest k)
-  end.
-
-Lemma index_of'_spec : forall k m, match index_of' m k with
-  | Some i => 0 <= i < Zlength m /\ (fst (Znth i m (0, 0)) = k \/ fst (Znth i m (0, 0)) = 0) /\
-              Forall (fun x => fst x <> 0 /\ fst x <> k) (sublist 0 i m)
-  | None => ~In k (map fst m) /\ ~In 0 (map fst m)
-  end.
-Proof.
-  induction m; simpl; auto; intros.
-  destruct a.
-  rewrite Zlength_cons.
-  pose proof (Zlength_nonneg m).
-  destruct (eq_dec z 0).
-  { subst; split; [omega|].
-    rewrite sublist_nil, Znth_cons_eq; split; auto. }
-  destruct (eq_dec z k).
-  { subst; split; [omega|].
-    rewrite sublist_nil, Znth_cons_eq; split; auto. }
-  destruct (index_of' m k); simpl.
-  - destruct IHm as (? & ? & ?); unfold Z.succ; rewrite Znth_cons_eq, Z.add_simpl_r.
-    split; [omega|].
-    if_tac; [omega|].
-    split; auto.
-    rewrite sublist_0_cons, Z.add_simpl_r by omega; constructor; auto.
-  - tauto.
-Qed.
-
-Lemma Znth_rebase : forall m i j d, 0 <= i < Zlength m -> 0 <= j < Zlength m ->
-  Znth i (rebase m j) d = Znth ((i + j) mod Zlength m) m d.
-Proof.
-  intros; unfold rebase.
-  destruct (eq_dec (Zlength m) 0); [omega|].
-  rewrite Znth_rotate by omega; f_equal.
-  rewrite Z.sub_sub_distr, <- Z.add_sub_swap.
-  replace (i + j - Zlength m) with (i + j + (-1 * Zlength m)) by omega.
-  rewrite Z.mod_add; auto.
-Qed.
-
-Corollary Znth_rebase' : forall m i j d, 0 <= i < Zlength m -> 0 <= j < Zlength m ->
-  Znth ((i - j) mod Zlength m) (rebase m j) d = Znth i m d.
-Proof.
-  intros; rewrite Znth_rebase; auto.
-  - rewrite Zplus_mod_idemp_l, Z.sub_simpl_r, Zmod_small; auto.
-  - apply Z_mod_lt; omega.
-Qed.
-
-Definition lookup (m : list (Z * Z)) (k : Z) :=
-  option_map (fun i => (i + hash k) mod 32) (index_of' (rebase m (hash k)) k).
-
-Definition set m k v := option_map (fun i => upd_Znth i m (k, v)) (lookup m k).
-
-Definition get m k := match lookup m k with Some i => let '(k', v') := Znth i m (0, 0) in
-  if eq_dec k' 0 then None else Some v' | None => None end.
-
-Lemma index_of'_upd : forall m k v i (Hrange : 0 <= i < Zlength m)
-  (Hi : fst (Znth i m (0, 0)) = k \/ fst (Znth i m (0, 0)) = 0),
-  index_of' (upd_Znth i m (k, v)) k = index_of' m k.
-Proof.
-  intros.
-  pose proof (index_of'_spec k m) as Hk; pose proof (index_of'_spec k (upd_Znth i m (k, v))) as Hk'.
-  destruct (index_of' m k), (index_of' (upd_Znth i m (k, v)) k); auto.
-  - rewrite upd_Znth_Zlength in Hk' by auto.
-    destruct Hk as (? & Hk & ?).
-    destruct Hk' as (? & Hz & Hall).
-    destruct (zlt i z0).
-    { rewrite sublist_upd_Znth_lr in Hall by omega.
-      rewrite Forall_forall in Hall; specialize (Hall _ (upd_Znth_In _ _ _)); tauto. }
-    rewrite sublist_upd_Znth_l in Hall by omega.
-    f_equal; destruct (eq_dec i z0); [subst | rewrite upd_Znth_diff' in Hz by auto];
-      eapply Forall_sublist_first; eauto; simpl; try omega.
-    + destruct Hi as [-> | ->]; tauto.
-    + destruct Hk as [-> | ->]; tauto.
-    + destruct Hz as [-> | ->]; tauto.
-    + destruct Hk as [-> | ->]; tauto.
-  - rewrite <- upd_Znth_map in Hk'; destruct Hk' as (Hk' & _); contradiction Hk'.
-    apply upd_Znth_In.
-  - destruct Hk as (Hk & Hz); destruct Hi; [contradiction Hk | contradiction Hz]; rewrite in_map_iff;
-      do 2 eexists; eauto; apply Znth_In; auto.
-Qed.
-
-Lemma hash_range : forall i, 0 <= hash i < 32.
-Proof.
-  intro; apply Z_mod_lt; computable.
-Qed.
-
-Lemma Zlength_rebase : forall m i, 0 <= i < Zlength m -> Zlength (rebase m i) = Zlength m.
-Proof.
-  intros; unfold rebase; rewrite Zlength_rotate; auto; omega.
-Qed.
-
-Lemma rebase_upd : forall m i j x, 0 <= i < Zlength m -> 0 <= j < Zlength m ->
-  rebase (upd_Znth i m x) j = upd_Znth ((i - j) mod Zlength m) (rebase m j) x.
-Proof.
-  intros; unfold rebase.
-  destruct (eq_dec (Zlength m) 0); [omega|].
-  rewrite upd_rotate; auto; try omega.
-  rewrite upd_Znth_Zlength by auto.
-  f_equal; f_equal.
-  rewrite Zminus_mod_idemp_l.
-  replace (i - j - (Zlength m - j)) with (i + (-1 * Zlength m)) by omega.
-  rewrite Z.mod_add, Zmod_small; auto.
-  { apply Z_mod_lt; omega. }
-Qed.
-
-Corollary rebase_upd' : forall m i j x, 0 <= i < Zlength m -> 0 <= j < Zlength m ->
-  rebase (upd_Znth ((i + j) mod Zlength m) m x) j = upd_Znth i (rebase m j) x.
-Proof.
-  intros; rewrite rebase_upd; auto.
-  - rewrite Zminus_mod_idemp_l, Z.add_simpl_r, Zmod_small; auto.
-  - apply Z_mod_lt; omega.
-Qed.
-
-Lemma lookup_set : forall m k v m', set m k v = Some m' -> Zlength m = 32 -> lookup m' k = lookup m k.
-Proof.
-  unfold set; intros.
-  destruct (lookup m k) eqn: Hlookup; [inv H | discriminate].
-  unfold lookup in *.
-  pose proof (hash_range k).
-  pose proof (index_of'_spec k (rebase m (hash k))) as Hspec.
-  destruct (index_of' (rebase m (hash k)) k) eqn: Hindex; [|discriminate].
-  simpl in Hlookup; inv Hlookup.
-  rewrite Zlength_rebase in Hspec by omega; destruct Hspec as (? & Hz & ?).
-  replace 32 with (Zlength m); rewrite rebase_upd' by (auto; omega).
-  rewrite index_of'_upd, Hindex; auto.
-  { rewrite Zlength_rebase; omega. }
-Qed.
-
-Lemma lookup_range : forall m k i, lookup m k = Some i -> Zlength m = 32 -> 0 <= i < Zlength m.
-Proof.
-  unfold lookup; intros.
-  pose proof (index_of'_spec k (rebase m (hash k))) as Hspec.
-  destruct (index_of' (rebase m (hash k)) k); [inv H | discriminate].
-  replace (Zlength m) with 32; apply Z_mod_lt; computable.
-Qed.
-
-Lemma index_of'_upd2 : forall m k i k' v' (Hrange : 0 <= i < Zlength m)
-  (Hi : index_of' m k <> Some i) (Hdiff : k' <> k /\ k' <> 0),
-  index_of' (upd_Znth i m (k', v')) k = index_of' m k.
-Proof.
-  intros.
-  pose proof (index_of'_spec k m) as Hk; pose proof (index_of'_spec k (upd_Znth i m (k', v'))) as Hk'.
-  destruct (index_of' m k), (index_of' (upd_Znth i m (k', v')) k); auto.
-  - rewrite upd_Znth_Zlength in Hk' by auto.
-    destruct Hk as (? & Hk & ?).
-    destruct Hk' as (? & Hz & Hall).
-    destruct (eq_dec z0 i).
-    { subst; rewrite upd_Znth_same in Hz by auto; tauto. }
-    rewrite upd_Znth_diff' in Hz by auto.
-    f_equal; apply Z.le_antisymm.
-    + eapply Forall_sublist_le; try eassumption; simpl; try omega.
-      { rewrite upd_Znth_Zlength; auto; omega. }
-      rewrite upd_Znth_diff' by auto.
-      destruct Hk as [-> | ->]; tauto.
-    + eapply Forall_sublist_le; try eassumption; simpl; try omega.
-      destruct Hz as [-> | ->]; tauto.
-  - destruct Hk as (? & Hk & ?).
-    erewrite <- upd_Znth_diff' with (j := i) in Hk by auto.
-    destruct Hk' as (Hk' & Hz'); destruct Hk; [contradiction Hk' | contradiction Hz'];
-      rewrite in_map_iff; do 2 eexists; eauto; apply Znth_In; rewrite upd_Znth_Zlength; auto.
-  - destruct Hk' as (Hrange' & Hz & ?).
-    destruct (eq_dec z i).
-    { subst; rewrite upd_Znth_same in Hz by auto; tauto. }
-    rewrite upd_Znth_Zlength in Hrange' by auto.
-    rewrite upd_Znth_diff' in Hz by auto.
-    destruct Hk as (Hk' & Hz'); destruct Hz; [contradiction Hk' | contradiction Hz'];
-      rewrite in_map_iff; do 2 eexists; eauto; apply Znth_In; auto.
-Qed.
-
-Lemma lookup_upd_diff : forall m k i k' v', lookup m k <> Some i -> Zlength m = 32 -> 0 <= i < Zlength m ->
-  k' <> k /\ k' <> 0 ->
-  lookup (upd_Znth i m (k', v')) k = lookup m k.
-Proof.
-  unfold lookup; intros.
-  pose proof (hash_range k).
-  rewrite rebase_upd by (auto; omega).
-  rewrite index_of'_upd2; auto.
-  - rewrite Zlength_rebase by omega.
-    apply Z_mod_lt; omega.
-  - intro X; rewrite X in H; simpl in H.
-    replace 32 with (Zlength m) in H.
-    rewrite Zplus_mod_idemp_l, Z.sub_simpl_r, Zmod_small in H by omega; contradiction H; auto.
-Qed.
-
-Lemma get_set_same : forall m k v m', set m k v = Some m' -> Zlength m = 32 -> k <> 0 ->
-  get m' k = Some v.
-Proof.
-  intros.
-  exploit lookup_set; eauto; intro Heq.
-  unfold set, get in *.
-  destruct (lookup m k) eqn: Hlookup; [inv H | discriminate].
-  exploit (lookup_range _ _ _ Hlookup); auto; intro.
-  rewrite Heq, upd_Znth_same by auto.
-  if_tac; [absurd (k = 0)|]; auto.
-Qed.
-
-Lemma get_override : forall m k v m' v', set m k v = Some m' -> Zlength m = 32 -> set m' k v' = set m k v'.
-Proof.
-  intros; unfold set.
-  exploit lookup_set; eauto; intros ->.
-  unfold set in H.
-  destruct (lookup m k) eqn: Hlookup; auto; inv H; simpl.
-  exploit lookup_range; eauto; intro.
-  rewrite upd_Znth_twice; auto.
-Qed.
-
-Lemma index_of_app : forall k m1 m2, index_of (m1 ++ m2) k =
-  match index_of m1 k with Some i => Some i | None => option_map (Z.add (Zlength m1)) (index_of m2 k) end.
-Proof.
-  induction m1; simpl; intros.
-  - destruct (index_of m2 k); auto.
-  - destruct a.
-    destruct (eq_dec z k); auto.
-    rewrite IHm1; destruct (index_of m1 k); auto; simpl.
-    destruct (index_of m2 k); auto; simpl.
-    rewrite Zlength_cons; f_equal; omega.
-Qed.
-
-Lemma index_of_out : forall k m, Forall (fun x => fst x <> k) m -> index_of m k = None.
-Proof.
-  intros.
-  pose proof (index_of_spec k m) as Hk.
-  destruct (index_of m k); auto.
-  destruct Hk as (? & ? & ?); eapply Forall_Znth in H; eauto.
-  subst; contradiction H; eauto.
-Qed.
-
-Lemma index_of_sublist : forall m a b i k (HNoDup : NoDup (map fst m))
-  (Hi : index_of (sublist a b m) k = Some i) (Ha : 0 <= a) (Hb : b <= Zlength m),
-  index_of m k = Some (i + a).
-Proof.
-  intros.
-  destruct (Z_le_dec b a); [rewrite sublist_nil_gen in Hi by auto; discriminate|].
-  assert (m = sublist 0 a m ++ sublist a b m ++ sublist b (Zlength m) m) as Hm.
-  { rewrite !sublist_rejoin, sublist_same; auto; omega. }
-  rewrite Hm, index_of_app, index_of_out, index_of_app, Hi; simpl.
-  rewrite Zlength_sublist by omega.
-  f_equal; omega.
-  { rewrite Hm, !map_app in HNoDup; apply NoDup_app in HNoDup.
-    destruct HNoDup as (_ & _ & HNoDup).
-    rewrite Forall_forall; intros ???.
-    exploit (HNoDup k); try contradiction.
-    * rewrite in_map_iff; eauto.
-    * rewrite in_app; left.
-      pose proof (index_of_spec k (sublist a b m)) as Hspec; rewrite Hi in Hspec.
-      destruct Hspec as (? & ? & ?).
-      rewrite in_map_iff; do 2 eexists; eauto.
-      apply Znth_In; auto. }
-Qed.
-
-Lemma index_of_rotate : forall m n k, 0 <= n <= Zlength m -> NoDup (map fst m) ->
-  index_of (rotate m n (Zlength m)) k = option_map (fun i => (i + n) mod Zlength m) (index_of m k).
-Proof.
-  intros.
-  destruct (eq_dec (Zlength m) 0).
-  { apply Zlength_nil_inv in e; subst.
-    unfold rotate; rewrite !sublist_of_nil; auto. }
-  unfold rotate; rewrite !index_of_app.
-  destruct (index_of (sublist (Zlength m - n) (Zlength m) m) k) eqn: Hk2.
-  - pose proof (index_of_spec k (sublist (Zlength m - n) (Zlength m) m)) as Hspec.
-    rewrite Hk2 in Hspec; destruct Hspec as (Hrange & ?).
-    apply index_of_sublist in Hk2; auto; try omega.
-    rewrite Hk2; simpl.
-    rewrite Zlength_sublist in Hrange by omega.
-    replace (z + _ + _) with (z + Zlength m) by omega.
-    rewrite Z.add_mod, Z_mod_same_full, Z.add_0_r, Zmod_mod by auto.
-    rewrite Zmod_small; auto; omega.
-  - replace (index_of m k) with
-      (index_of (sublist 0 (Zlength m - n) m ++ sublist (Zlength m - n) (Zlength m) m) k)
-      by (rewrite sublist_rejoin, sublist_same; auto; omega).
-    rewrite index_of_app, Hk2.
-    pose proof (index_of_spec k (sublist 0 (Zlength m - n) m)) as Hspec.
-    destruct (index_of (sublist 0 (Zlength m - n) m) k); auto; simpl.
-    rewrite Zlength_sublist in Hspec by omega.
-    rewrite Zlength_sublist, Zmod_small by omega.
-    f_equal; omega.
-Qed.
-
-Corollary index_of_rebase : forall m n k, 0 <= n <= Zlength m -> NoDup (map fst m) ->
-  index_of (rebase m n) k = option_map (fun i => (i - n) mod Zlength m) (index_of m k).
-Proof.
-  intros; unfold rebase.
-  destruct (eq_dec (Zlength m) 0).
-  { apply Zlength_nil_inv in e; subst.
-    rewrite rotate_nil; auto. }
-  rewrite index_of_rotate by (auto; omega).
-  destruct (index_of m k); auto; simpl.
-  replace (z + (Zlength m - n)) with (z - n + (1 * Zlength m)) by omega.
-  rewrite Z.mod_add; auto.
-Qed.
-
-Lemma index_of'_succeeds : forall k m i (Hi : 0 <= i < Zlength m)
-  (Hnz : Forall (fun x => fst x <> 0 /\ fst x <> k) (sublist 0 i m))
-  (Hk : fst (Znth i m (0, 0)) = k \/ fst (Znth i m (0, 0)) = 0), index_of' m k = Some i.
-Proof.
-  intros.
-  pose proof (index_of'_spec k m).
-  destruct (index_of' m k).
-  - destruct H as (? & Hz & Hnz').
-    f_equal; eapply Forall_sublist_first with (d := (0, 0)); eauto; omega.
-  - destruct H as (Hk' & Hz'); destruct Hk; [contradiction Hk' | contradiction Hz'];
-      rewrite in_map_iff; do 2 eexists; eauto; apply Znth_In; auto.
-Qed.
-
-Lemma lookup_spec : forall m k (Hwf : wf_map m) (Hchain : well_chained m) (Hlen : Zlength m = 32)
-  (Hnz : k <> 0) (Hin : In k (map fst m)), lookup m k = index_of m k.
-Proof.
-  intros.
-  destruct (eq_dec (Zlength m) 0).
-  { apply Zlength_nil_inv in e; subst; contradiction. }
-  specialize (Hchain k).
-  pose proof (hash_range k).
-  assert (0 <= hash k <= Zlength m) by omega.
-  rewrite index_of_rebase in Hchain by auto.
-  unfold lookup.
-  pose proof (index_of_spec k m) as Hspec; destruct (index_of m k) eqn: Hk; [|contradiction].
-  specialize (Hchain _ eq_refl).
-  destruct Hspec as (? & Hz & ?).
-  assert (0 <= (z - hash k) mod Zlength m < Zlength m) by (apply Z_mod_lt; omega).
-  assert (((z - hash k) mod Zlength m + hash k) mod Zlength m = z) as Hmod.
-  { rewrite Zplus_mod_idemp_l, Z.sub_simpl_r, Zmod_small; auto. }
-  assert (fst (Znth ((z - hash k) mod Zlength m) (rebase m (hash k)) (0, 0)) = k).
-  { rewrite Znth_rebase, Hmod; auto; omega. }
-  erewrite index_of'_succeeds; eauto; simpl.
-  rewrite <- Hlen, Hmod; auto.
-  + rewrite Zlength_rebase; auto; omega.
-  + rewrite Forall_forall; intros ? Hin'.
-    split; [rewrite Forall_forall in Hchain; apply Hchain; rewrite !Hlen in *; auto|].
-    intro Heq; apply In_Znth with (d := (0, 0)) in Hin'.
-    destruct Hin' as (i & Hi & ?); subst x.
-    rewrite Zlength_sublist in Hi; try omega.
-    rewrite Znth_sublist, Znth_rebase, Z.add_0_r in Heq by omega.
-    eapply NoDup_Znth_inj with (i0 := z)(j := (i + hash k) mod (Zlength m)) in Hwf.
-    subst z.
-    rewrite Zminus_mod_idemp_l, Z.add_simpl_r, Z.sub_0_r, Zmod_small in Hi; try omega.
-    * destruct Hi; split; auto.
-      etransitivity; eauto.
-      apply Z_mod_lt; omega.
-    * rewrite Zlength_map; auto.
-    * rewrite Zlength_map; apply Z_mod_lt; omega.
-    * rewrite !Znth_map'; subst k; eauto.
-    * rewrite Zlength_rebase; omega.
-Qed.
-
-(* Some of these should probably go up to ghost, or at least atomics. *)
-Definition value_of e :=
-  match e with
-  | Load v => v
-  | Store v => v
-  | CAS r c w => if eq_dec r c then w else r
-  end.
-
-Definition last_value (h : hist) v :=
-  (* initial condition *)
-  (h = [] /\ v = vint 0) \/
-  exists n e, In (n, e) h /\ value_of e = v /\ Forall (fun x => let '(m, _) := x in m <= n)%nat h.
-
-Definition newer (l : hist) t := Forall (fun x => fst x < t)%nat l.
-
-Lemma last_value_new : forall h n e, newer h n ->
-  last_value (h ++ [(n, e)]) (value_of e).
-Proof.
-  right.
-  do 3 eexists; [rewrite in_app; simpl; eauto|].
-  rewrite Forall_app; repeat constructor.
-  eapply Forall_impl; [|eauto]; intros.
-  destruct a; simpl in *; omega.
-Qed.
-
-Definition ordered_hist h := forall i j (Hi : 0 <= i < j) (Hj : j < Zlength h),
-  (fst (Znth i h (O, Store (vint 0))) < fst (Znth j h (O, Store (vint 0))))%nat.
-
-Lemma ordered_cons : forall t e h, ordered_hist ((t, e) :: h) ->
-  Forall (fun x => let '(m, _) := x in t < m)%nat h /\ ordered_hist h.
-Proof.
-  unfold ordered_hist; split.
-  - rewrite Forall_forall; intros (?, ?) Hin.
-    apply In_Znth with (d := (O, Store (vint 0))) in Hin.
-    destruct Hin as (j & ? & Hj).
-    exploit (H 0 (j + 1)); try omega.
-    { rewrite Zlength_cons; omega. }
-    rewrite Znth_0_cons, Znth_pos_cons, Z.add_simpl_r, Hj by omega; auto.
-  - intros; exploit (H (i + 1) (j + 1)); try omega.
-    { rewrite Zlength_cons; omega. }
-    rewrite !Znth_pos_cons, !Z.add_simpl_r by omega; auto.
-Qed.
-
-Lemma ordered_last : forall t e h (Hordered : ordered_hist h) (Hin : In (t, e) h)
-  (Ht : Forall (fun x => let '(m, _) := x in m <= t)%nat h), last h (O, Store (vint 0)) = (t, e).
-Proof.
-  induction h; [contradiction | simpl; intros].
-  destruct a; apply ordered_cons in Hordered; destruct Hordered as (Ha & ?).
-  inversion Ht as [|??? Hp]; subst.
-  destruct Hin as [Hin | Hin]; [inv Hin|].
-  - destruct h; auto.
-    inv Ha; inv Hp; destruct p; omega.
-  - rewrite IHh; auto.
-    destruct h; auto; contradiction.
-Qed.
-
-Definition value_of_hist (h : hist) := value_of (snd (last h (O, Store (vint 0)))).
-
-Lemma ordered_last_value : forall h v (Hordered : ordered_hist h), last_value h v <-> value_of_hist h = v.
-Proof.
-  unfold last_value, value_of_hist; split; intro.
-  - destruct H as [(? & ?) | (? & ? & ? & ? & ?)]; subst; auto.
-    erewrite ordered_last; eauto; auto.
-  - destruct h; [auto | right].
-    destruct (last (p :: h) (O, Store (vint 0))) as (t, e) eqn: Hlast.
-    exploit (@app_removelast_last _ (p :: h)); [discriminate | intro Heq].
-    rewrite Hlast in Heq.
-    exists t; exists e; repeat split; auto.
-    + rewrite Heq, in_app; simpl; auto.
-    + unfold ordered_hist in Hordered.
-      rewrite Forall_forall; intros (?, ?) Hin.
-      apply In_Znth with (d := (O, Store (vint 0))) in Hin.
-      destruct Hin as (i & ? & Hi).
-      rewrite <- Znth_last in Hlast.
-      destruct (eq_dec i (Zlength (p :: h) - 1)).
-      * subst; rewrite Hlast in Hi; inv Hi; auto.
-      * exploit (Hordered i (Zlength (p :: h) - 1)); try omega.
-        rewrite Hlast, Hi; simpl; omega.
-Qed.
-
-Lemma newer_trans : forall l t1 t2, newer l t1 -> (t1 <= t2)%nat -> newer l t2.
-Proof.
-  intros.
-  eapply Forall_impl, H; simpl; intros; omega.
-Qed.
-
-Corollary newer_snoc : forall l t1 e t2, newer l t1 -> (t1 < t2)%nat -> newer (l ++ [(t1, e)]) t2.
-Proof.
-  unfold newer; intros.
-  rewrite Forall_app; split; [|repeat constructor; auto].
-  eapply newer_trans; eauto; omega.
-Qed.
-
-Lemma ordered_snoc : forall h t e, ordered_hist h -> newer h t -> ordered_hist (h ++ [(t, e)]).
-Proof.
-  repeat intro.
-  rewrite Zlength_app, Zlength_cons, Zlength_nil in Hj.
-  rewrite app_Znth1 by omega.
-  destruct (eq_dec j (Zlength h)).
-  - rewrite Znth_app1; auto.
-    apply Forall_Znth; auto; omega.
-  - specialize (H i j).
-    rewrite app_Znth1 by omega; apply H; auto; omega.
-Qed.
-
-Definition int_op e :=
-  match e with
-  | Load v | Store v => tc_val tint v
-  | CAS r c w => tc_val tint r /\ tc_val tint c /\ tc_val tint w
-  end.
+  - computable.
+  - intro; apply Z_mod_lt; computable.
+Defined.
 
 (* Once set, a key is never reset. *)
 Definition k_R (h : list hist_el) (v : val) := !!(Forall int_op h /\
@@ -560,63 +35,12 @@ Definition k_R (h : list hist_el) (v : val) := !!(Forall int_op h /\
 
 Definition v_R (h : list hist_el) (v : val) := emp.
 
-Definition atomic_entry sh p := !!(field_compatible tentry [] p) && EX lkey : val, EX lval : val,
-  field_at sh tentry [StructField _lkey] lkey p *
-  atomic_loc sh lkey (field_address tentry [StructField _key] p) (vint 0) Tsh k_R *
-  field_at sh tentry [StructField _lvalue] lval p *
-  atomic_loc sh lval (field_address tentry [StructField _value] p) (vint 0) Tsh v_R.
-
 (* Entries are no longer consecutive. *)
 Definition wf_hists h := Forall (fun x => (ordered_hist (fst x) /\ Forall int_op (map snd (fst x))) /\
   (ordered_hist (snd x) /\ Forall int_op (map snd (snd x)))) h.
 
-Definition make_int v := match v with Vint i => Int.signed i | _ => 0 end.
-
-Lemma make_int_spec : forall v, tc_val tint v -> vint (make_int v) = v.
-Proof.
-  destruct v; try contradiction; simpl.
-  rewrite Int.repr_signed; auto.
-Qed.
-
-Lemma make_int_repable : forall v, repable_signed (make_int v).
-Proof.
-  destruct v; simpl; try (split; computable).
-  apply Int.signed_range.
-Qed.
-
 Definition make_map h :=
   map (fun hs => (make_int (value_of_hist (fst hs)), make_int (value_of_hist (snd hs)))) h.
-
-Lemma make_map_eq : forall h h', Forall2 (fun a b => value_of_hist (fst a) = value_of_hist (fst b) /\
-  value_of_hist (snd a) = value_of_hist (snd b)) h h' -> make_map h = make_map h'.
-Proof.
-  induction 1; auto; simpl.
-  destruct x, y; simpl in *.
-  destruct H as (-> & ->); rewrite IHForall2; auto.
-Qed.
-
-Lemma int_op_value : forall e, int_op e -> tc_val tint (value_of e).
-Proof.
-  destruct e; auto; simpl.
-  intros (? & ? & ?); destruct (eq_dec r c); auto.
-Qed.
-
-Corollary int_op_value_of_hist : forall h, Forall int_op (map snd h) -> tc_val tint (value_of_hist h).
-Proof.
-  intros; unfold value_of_hist.
-  apply Forall_last; simpl; auto.
-  rewrite Forall_map in H; eapply Forall_impl; [|eauto].
-  simpl; intros; apply int_op_value; auto.
-Qed.
-
-Lemma make_map_no_key : forall h k (Hout : Forall (fun x => make_int (value_of_hist (fst x)) <> k) h),
-  Forall (fun x => fst x <> k) (make_map h).
-Proof.
-  induction h; simpl; auto; intros.
-  destruct a.
-  inv Hout.
-  constructor; auto.
-Qed.
 
 Definition failed_CAS k (a b : hist * hist) := exists t r, newer (fst a) t /\
   (fst b = fst a ++ [(t, Load (Vint r))] \/
@@ -636,149 +60,27 @@ Definition set_item_trace (h : list (hist * hist)) k v i h' := Zlength h' = Zlen
   forall j, (In j (indices (hash k) i) -> failed_CAS k (Znth j h ([], [])) (Znth j h' ([], []))) /\
     (~In j (indices (hash k) i) -> j <> i -> Znth j h' ([], []) = Znth j h ([], [])).
 
-Definition map_incl (m m' : list (Z * Z)) := forall k v i, k <> 0 -> Znth i m (0, 0) = (k, v) ->
-  Znth i m' (0, 0) = (k, v).
+Definition atomic_entry sh pk pv hk hv :=
+  atomic_loc sh pk (vint 0) k_R hk * atomic_loc sh pv (vint 0) v_R hv.
 
-(* It would be nice if we could maintain the invariant that the map has no duplicates and is well-chained,
-   and indeed, the algorithm should maintain these properties. However, the per-slot histories do not obviously
-   present a way to prove this: if a new key has "mysteriously appeared" (i.e., been added by another thread),
-   we don't have a good way of knowing that it's well-chained. *)
-(* We can, however, allow for the possibility that there is garbage in the map, and consider the abstract map
-   to be those elements that can be successfully looked up, rather than all pairs in the map. In practice, this
-   *should* come down to the same thing, but how could we prove it? *)
-Lemma set_item_trace_map : forall h k v i h' (Hwf : wf_hists h) (Hlenh : Zlength h = 32)
-  (Htrace : set_item_trace h k v i h') (Hk : k <> 0) (Hrepk : repable_signed k) (Hrepv : repable_signed v),
-  wf_hists h' /\ let m' := make_map (upd_Znth i h' (Znth i h ([], []))) in
-    map_incl (make_map h) m' /\ set m' k v = Some (make_map h').
-Proof.
-  intros.
-  destruct Htrace as (Hlen & Hbounds & Hi & Hrest).
-  destruct (Znth i h ([], [])) as (hk, hv) eqn: Hhi.
-  destruct Hi as (t & r & tv & Ht & Htv & Hi1 & Hi2 & Hr0).
-  assert (i <= Zlength h') by (rewrite Hlen; destruct Hbounds; apply Z.lt_le_incl; auto).
-  assert (0 <= i + 1 <= Zlength h').
-  { rewrite Hlen; destruct Hbounds; split; [|rewrite <- lt_le_1]; auto; omega. }
-  assert (vint k <> vint 0).
-  { intro; contradiction Hk; apply repr_inj_signed; auto.
-    { split; computable. }
-    { congruence. }}
-  assert (r = vint 0 \/ r = vint k) as Hr.
-  { destruct Hi1 as [(? & ?) | (? & ? & ? & ?)]; auto. }
-  assert ((if eq_dec r (vint 0) then vint k else r) = vint k) as Hif.
-  { if_tac; auto.
-    destruct Hr; [absurd (r = vint 0)|]; auto. }
-  assert (value_of_hist (fst (Znth i h' ([], []))) = vint k) as Hk'.
-  { destruct Hi1 as [(-> & ?) | (? & ? & -> & ?)].
-    - unfold value_of_hist; rewrite last_snoc; auto.
-    - rewrite app_cons_assoc; unfold value_of_hist; rewrite last_snoc; auto. }
-  assert (wf_hists h') as Hwf'; [|split; auto; split].
-  - unfold wf_hists; rewrite Forall_forall_Znth; intros j ?.
-    apply (Forall_Znth _ _ j ([], [])) in Hwf; [destruct Hwf as ((? & ?) & ? & ?) | omega].
-    destruct (eq_dec j i); [|specialize (Hrest j); destruct (in_dec Z_eq_dec j (indices (hash k) i))].
-    + subst; rewrite Hhi in *.
-      split; [|rewrite Hi2, map_app, Forall_app; repeat constructor; auto; apply ordered_snoc; auto].
-      destruct Hi1 as [(-> & _) | (? & ? & -> & _)]; rewrite map_app, Forall_app; repeat constructor;
-        auto; try (apply ordered_snoc; auto).
-      * rewrite app_cons_assoc; apply ordered_snoc; [apply ordered_snoc; auto|].
-        apply newer_snoc; auto.
-      * destruct Hr; subst; simpl; auto.
-    + destruct Hrest as ((? & ? & ? & Hcase & ? & ? & -> & ?) & _); auto; simpl in *.
-      split; auto.
-      destruct Hcase as [-> | (? & ? & ->)]; rewrite map_app, Forall_app; repeat constructor; auto.
-      * apply ordered_snoc; auto.
-      * rewrite app_cons_assoc; apply ordered_snoc; [apply ordered_snoc; auto|].
-        apply newer_snoc; auto.
-    + destruct Hrest as (_ & ->); auto.
-  - intros k0 v0 j Hk0 Hj.
-    exploit (Znth_inbounds j (make_map h) (0, 0)).
-    { rewrite Hj; intro X; inv X; contradiction Hk0; auto. }
-    intro; unfold make_map in *; rewrite <- upd_Znth_map.
-    rewrite Zlength_map in *.
-    rewrite Znth_map with (d' := ([], [])) in Hj by auto; inv Hj.
-    destruct (eq_dec j i); [subst; rewrite upd_Znth_same, Hhi; auto | rewrite upd_Znth_diff'];
-      rewrite ?Zlength_map in *; auto; try omega.
-    rewrite Znth_map with (d' := ([], [])) by omega.
-    specialize (Hrest j); destruct (in_dec Z_eq_dec j (indices (hash k) i));
-      [|destruct Hrest as (_ & ->); auto].
-    destruct Hrest as ((? & r1 & ? & Hcase & ? & ? & -> & Heq) & _); auto; simpl in *.
-    assert (value_of_hist (fst (Znth j h ([], []))) <> vint 0).
-    { intro X; rewrite X in Hk0; contradiction Hk0; auto. }
-    destruct Hcase as [-> | (? & ? & ->)].
-    + unfold value_of_hist at 1; rewrite last_snoc, Heq; auto.
-    + rewrite app_cons_assoc; unfold value_of_hist at 1; rewrite last_snoc, Heq; auto; simpl.
-      destruct (eq_dec (Vint r1) (vint 0)); auto.
-      absurd (r1 = Int.zero); auto; inv e; auto.
-  - assert (0 <= i < Zlength h') by (rewrite Hlen; auto).
-    unfold set.
-    assert (lookup (make_map (upd_Znth i h' (hk, hv))) k = Some i) as ->.
-    + unfold lookup, make_map.
-      assert (i = ((i - hash k) mod 32 + hash k) mod 32) as Hmod.
-      { rewrite Zplus_mod_idemp_l, Z.sub_simpl_r, Zmod_small by omega; auto. }
-      pose proof (hash_range k).
-      assert (Zlength (map (fun hs => (make_int (value_of_hist (fst hs)), make_int (value_of_hist (snd hs))))
-              (upd_Znth i h' (hk, hv))) = 32) as Hlen1.
-      { rewrite Zlength_map, upd_Znth_Zlength; auto; omega. }
-      erewrite index_of'_succeeds; simpl.
-      f_equal; symmetry; apply Hmod.
-      { rewrite Zlength_rebase; rewrite ?Zlength_map, ?upd_Znth_Zlength; auto; try omega.
-        replace (Zlength h') with 32; [apply Z_mod_lt; computable | omega]. }
-      { rewrite Forall_forall; intros x Hin.
-        apply In_Znth with (d := (0, 0)) in Hin; destruct Hin as (j & Hj & Hx).
-        exploit (Z_mod_lt (i - hash k) 32); [computable | intro].
-        rewrite Zlength_sublist in Hj; rewrite ?Zlength_rebase; rewrite ?Hlen1; try omega.
-        rewrite Znth_sublist, Z.add_0_r in Hx by (auto; omega).
-        rewrite Znth_rebase in Hx by omega.
-        rewrite Hlen1, Znth_map with (d' := ([], [])) in Hx.
-        subst x; simpl.
-        specialize (Hrest ((j + hash k) mod 32)); destruct Hrest as ((? & r1 & ? & Hcase & ? & ? & ?) & _).
-        { unfold indices; rewrite in_map_iff.
-          exists j; split; [rewrite Z.add_comm; auto|].
-          rewrite In_upto, Z2Nat.id; omega. }
-        rewrite upd_Znth_diff'; auto.
-        destruct Hcase as [-> | (? & ? & ->)]; [|rewrite app_cons_assoc]; unfold value_of_hist;
-          rewrite last_snoc; simpl.
-        * split; intro X; [absurd (r1 = Int.zero) | absurd (r1 = Int.repr k)]; auto; apply signed_inj; auto.
-          rewrite Int.signed_repr; auto.
-        * destruct (eq_dec (Vint r1) (vint 0)); [absurd (r1 = Int.zero); auto; inversion e; auto | simpl].
-          split; intro X; [absurd (r1 = Int.zero) | absurd (r1 = Int.repr k)]; auto; apply signed_inj; auto.
-          rewrite Int.signed_repr; auto.
-        * intro X; rewrite <- X, Zminus_mod_idemp_l, Z.add_simpl_r, Z.sub_0_r, Zmod_small in Hj; try omega.
-          destruct Hj; split; auto; etransitivity; eauto; apply Z_mod_lt; computable.
-        * rewrite upd_Znth_Zlength by auto.
-          replace (Zlength h') with 32 by omega; apply Z_mod_lt; computable. }
-      { rewrite <- Hlen1, Znth_rebase', Znth_map with (d' := ([], [])); simpl;
-          rewrite ?Zlength_map, ?upd_Znth_Zlength; auto; try omega.
-        rewrite upd_Znth_same by auto; simpl.
-        destruct (eq_dec (value_of_hist hk) (vint 0)); [rewrite e; auto|].
-        rewrite Hr0; auto; destruct Hr; subst r; auto; simpl.
-        rewrite Int.signed_repr; auto. }
-    + simpl; unfold make_map; erewrite <- upd_Znth_map, upd_Znth_twice, upd_Znth_triv; rewrite ?Zlength_map;
-        auto.
-      rewrite Znth_map', Hk', Hi2.
-      unfold value_of_hist; rewrite last_snoc; simpl.
-      rewrite !Int.signed_repr; auto.
-Qed.
+Definition atomic_entries sh entries hists := fold_right sepcon emp
+  (map (fun x => let '((pk, pv), (hk, hv)) := x in atomic_entry sh pk pv hk hv) (combine entries hists)).
 
 (* What can a thread know?
    At least certain keys exist, and whatever it did last took effect.
    It can even rely on the indices of known keys. *)
 Definition set_item_spec :=
  DECLARE _set_item
-  WITH key : Z, value : Z, p : val, sh : share, entries : list val, h : list (hist * hist)
+  WITH key : Z, value : Z, p : val, sh : share, entries : list (val * val), h : list (hist * hist)
   PRE [ _key OF tint, _value OF tint ]
-   PROP (repable_signed key; repable_signed value; readable_share sh; key <> 0; Forall isptr entries;
-         Zlength h = 32; wf_hists h)
+   PROP (repable_signed key; repable_signed value; readable_share sh; key <> 0; Zlength h = size; wf_hists h)
    LOCAL (temp _key (vint key); temp _value (vint value); gvar _m_entries p)
-   SEP (data_at sh (tarray (tptr tentry) 32) entries p;
-        fold_right sepcon emp (map (atomic_entry sh) entries);
-        entry_hists entries h)
+   SEP (data_at sh (tarray tentry size) entries p; atomic_entries sh entries h)
   POST [ tvoid ]
    EX i : Z, EX h' : list (hist * hist),
    PROP (set_item_trace h key value i h')
    LOCAL ()
-   SEP (data_at sh (tarray (tptr tentry) 32) entries p;
-        fold_right sepcon emp (map (atomic_entry sh) entries);
-        entry_hists entries h').
+   SEP (data_at sh (tarray tentry size) entries p; atomic_entries sh entries h').
 (* set_item_trace_map describes the properties on the resulting map. *)
 
 (*Lemma index_of_iff_out : forall m k, index_of m k = None <-> ~In k (map fst m).
@@ -821,165 +123,22 @@ Definition get_item_trace (h : list (hist * hist)) k v i h' := Zlength h' = Zlen
   forall j, (In j (indices (hash k) i) -> failed_load k (Znth j h ([], [])) (Znth j h' ([], []))) /\
     (~In j (indices (hash k) i) -> j <> i -> Znth j h' ([], []) = Znth j h ([], [])).
 
-Lemma get_item_trace_map : forall h k v i h' (Hwf : wf_hists h) (Hlenh : Zlength h = 32)
-  (Htrace : get_item_trace h k v i h') (Hk : k <> 0) (Hrepk : repable_signed k) (Hrepv : repable_signed v),
-  wf_hists h' /\ match get (make_map h') k with
-  | Some v' => v' = v /\ map_incl (upd_Znth i (make_map h) (k, v)) (make_map h')
-  | None => v = 0 /\ map_incl (make_map h) (make_map h') end.
-Proof.
-  intros.
-  destruct Htrace as (Hlen & Hbounds & Hi & Hrest).
-  destruct (Znth i h ([], [])) as (hk, hv) eqn: Hhi.
-  destruct Hi as (t & r & Ht & Hi1 & Hi2 & Hr0).
-  assert (i <= Zlength h') by (rewrite Hlen; destruct Hbounds; apply Z.lt_le_incl; auto).
-  assert (0 <= i + 1 <= Zlength h').
-  { rewrite Hlen; destruct Hbounds; split; [|rewrite <- lt_le_1]; auto; omega. }
-  assert (vint k <> vint 0).
-  { intro; contradiction Hk; apply repr_inj_signed; auto.
-    { split; computable. }
-    { congruence. }}
-  assert (wf_hists h') as Hwf'; [|split; auto].
-  - unfold wf_hists; rewrite Forall_forall_Znth; intros j ?.
-    apply (Forall_Znth _ _ j ([], [])) in Hwf; [destruct Hwf as ((? & ?) & ? & ?) | omega].
-    destruct (eq_dec j i); [|specialize (Hrest j); destruct (in_dec Z_eq_dec j (indices (hash k) i))].
-    + subst; rewrite Hhi in *.
-      split; [rewrite Hi1, map_app, Forall_app; repeat constructor; auto; apply ordered_snoc; auto|].
-      destruct Hi2 as [(? & ? & ->) | (? & ? & ? & ->)]; auto.
-      rewrite map_app, Forall_app; repeat constructor; auto; apply ordered_snoc; auto.
-    + destruct Hrest as ((? & ? & ? & -> & ? & ? & -> & ?) & _); auto; simpl in *.
-      split; auto.
-      rewrite map_app, Forall_app; repeat constructor; auto.
-      apply ordered_snoc; auto.
-    + destruct Hrest as (_ & ->); auto.
-  - unfold get, lookup.
-    pose proof (index_of'_spec k (rebase (make_map h') (hash k))) as Hspec.
-    destruct (index_of' (rebase (make_map h') (hash k)) k) eqn: Hindex; simpl.
-    unfold make_map at 1; rewrite Znth_map with (d' := ([], [])).
-    pose proof (hash_range k).
-    assert ((z + hash k) mod 32 = i) as Hz.
-    { destruct Hspec as (Hz & Hcase & Hall).
-      assert (Zlength (make_map h') = Zlength h') as Hlenm by (unfold make_map; rewrite Zlength_map; auto).
-      assert (z <= (i - hash k) mod Zlength (make_map h')) as Hle.
-      { eapply Forall_sublist_le; try apply Hall; simpl.
-        { apply Z_mod_lt; omega. }
-        { omega. }
-        rewrite Znth_rebase' by omega.
-        unfold make_map; rewrite Znth_map'.
-        rewrite Hi1; unfold value_of_hist; rewrite last_snoc; simpl.
-        destruct Hi2 as [(? & ? & ?) | (? & ?)]; subst; [|rewrite Int.signed_repr by auto]; tauto. }
-      rewrite Zlength_rebase in Hz by omega.
-      rewrite Znth_rebase, Hlenm in Hcase by omega.
-      unfold make_map in Hcase; rewrite Znth_map with (d' := ([], [])) in Hcase; simpl in Hcase.
-      destruct (eq_dec ((z + hash k) mod 32) i); auto.
-      specialize (Hrest ((z + hash k) mod 32)); destruct Hrest as ((? & r1 & ? & Hfst & ? & ? & ?) & _).
-      { unfold indices.
-        rewrite in_map_iff.
-        exists z; split; [rewrite Z.add_comm; auto|].
-        rewrite In_upto, Z2Nat.id.
-        rewrite Hlenm in Hle; replace (Zlength h') with 32 in Hle by omega.
-        destruct (eq_dec z ((i - hash k) mod 32)); [|omega].
-        contradiction n; rewrite e, Zplus_mod_idemp_l, Z.sub_simpl_r, Zmod_small; auto; omega.
-        { apply Z_mod_lt; computable. } }
-      replace (Zlength h') with 32 in Hcase by omega.
-      rewrite Hfst in Hcase; unfold value_of_hist in Hcase; rewrite last_snoc in Hcase; simpl in Hcase.
-      destruct Hcase; [absurd (r1 = Int.repr k) | absurd (r1 = Int.zero)]; auto; apply signed_inj; auto.
-      rewrite Int.signed_repr; auto.
-      { apply Z_mod_lt; omega. } }
-    rewrite Hz, Hi1.
-    replace (value_of_hist (hk ++ _)) with (vint r) by (unfold value_of_hist; rewrite last_snoc; auto); simpl.
-    destruct Hi2 as [(? & ? & Hi2) | (? & ? & ? & Hi2)]; rewrite Hi2; clear dependent z; subst; simpl.
-    + split; auto.
-      intros k0 v0 j Hk0 Hj.
-      exploit (Znth_inbounds j (make_map h) (0, 0)).
-      { rewrite Hj; intro X; inv X; contradiction Hk0; auto. }
-      unfold make_map in *; rewrite Zlength_map; intro;
-        rewrite Znth_map with (d' := ([], [])) in Hj by auto; inv Hj.
-      rewrite Znth_map with (d' := ([], [])) by omega.
-      destruct (eq_dec j i).
-      { subst; rewrite Hhi in *; simpl in *; contradiction Hk0.
-        destruct (eq_dec (value_of_hist hk) (vint 0)); [rewrite e; auto|].
-        rewrite Hr0; auto. }
-      specialize (Hrest j); destruct (in_dec Z_eq_dec j (indices (hash k) i)).
-      * destruct Hrest as ((? & ? & ? & -> & ? & ? & -> & Heq) & _); auto.
-        unfold value_of_hist at 1; rewrite last_snoc; simpl.
-        destruct (eq_dec (value_of_hist (fst (Znth j h ([], [])))) (vint 0));
-          [contradiction Hk0; rewrite e; auto|].
-        rewrite Heq; auto.
-      * destruct Hrest as (_ & ->); auto.
-    + unfold value_of_hist; rewrite last_snoc; simpl.
-      rewrite !Int.signed_repr by auto.
-      if_tac; [contradiction Hk; auto|].
-      split; auto.
-      intros k0 v0 j Hk0 Hj.
-      exploit (Znth_inbounds j (upd_Znth i (make_map h) (k, v)) (0, 0)).
-      { rewrite Hj; intro X; inv X; contradiction Hk0; auto. }
-      unfold make_map in *; rewrite upd_Znth_Zlength; rewrite Zlength_map; auto.
-      intro; rewrite Znth_map with (d' := ([], [])) by omega.
-      destruct (eq_dec j i).
-      { subst; rewrite upd_Znth_same in Hj by (rewrite Zlength_map; auto).
-        inv Hj; rewrite Hi1, Hi2.
-        unfold value_of_hist; rewrite !last_snoc; simpl.
-        rewrite !Int.signed_repr; auto. }
-      rewrite upd_Znth_diff' in Hj; rewrite ?Zlength_map; auto.
-      rewrite Znth_map with (d' := ([], [])) in Hj by auto; inv Hj.
-      specialize (Hrest j); destruct (in_dec Z_eq_dec j (indices (hash k) i)).
-      * destruct Hrest as ((? & ? & ? & -> & ? & ? & -> & Heq) & _); auto.
-        unfold value_of_hist at 1; rewrite last_snoc; simpl.
-        destruct (eq_dec (value_of_hist (fst (Znth j h ([], [])))) (vint 0));
-          [contradiction Hk0; rewrite e; auto|].
-        rewrite Heq; auto.
-      * destruct Hrest as (_ & ->); auto.
-    + replace (Zlength h') with 32 by omega; apply Z_mod_lt; computable.
-    + assert (In r (map fst (rebase (make_map h') (hash k)))).
-      { rewrite in_map_iff.
-        unfold rebase, make_map; eexists; rewrite rotate_In, in_map_iff.
-        split; [|do 2 eexists; eauto; apply Znth_In with (i0 := i); omega].
-        rewrite Hi1; unfold value_of_hist; rewrite last_snoc; simpl.
-        apply Int.signed_repr; destruct Hi2 as [(? & ? & ?) | (? & ?)]; subst; auto.
-        { pose proof (hash_range k).
-          rewrite Zlength_map; omega. } }
-      destruct Hspec as (Hnk & Hnz), Hi2 as [(? & ? & ?) | (? & ?)]; subst;
-        [contradiction Hnz | contradiction Hnk].
-Qed.
-
 (* Read the most recently written value. *)
 Definition get_item_spec :=
  DECLARE _get_item
-  WITH key : Z, p : val, sh : share, entries : list val, h : list (hist * hist)
+  WITH key : Z, p : val, sh : share, entries : list (val * val), h : list (hist * hist)
   PRE [ _key OF tint, _value OF tint ]
-   PROP (repable_signed key; readable_share sh; key <> 0; Forall isptr entries; Zlength h = 32; wf_hists h)
+   PROP (repable_signed key; readable_share sh; key <> 0; Zlength h = size; wf_hists h)
    LOCAL (temp _key (vint key); gvar _m_entries p)
-   SEP (data_at sh (tarray (tptr tentry) 32) entries p;
-        fold_right sepcon emp (map (atomic_entry sh) entries);
-        entry_hists entries h)
+   SEP (data_at sh (tarray tentry size) entries p; atomic_entries sh entries h)
   POST [ tint ]
    EX value : Z, EX i : Z, EX h' : list (hist * hist),
    PROP (repable_signed value; get_item_trace h key value i h')
    LOCAL (temp ret_temp (vint value))
-   SEP (data_at sh (tarray (tptr tentry) 32) entries p;
-        fold_right sepcon emp (map (atomic_entry sh) entries);
-        entry_hists entries h').
+   SEP (data_at sh (tarray tentry size) entries p; atomic_entries sh entries h').
 
-Definition Gprog : funspecs := ltac:(with_library prog [surely_malloc_spec; atomic_CAS_spec; atomic_load_spec;
-  atomic_store_spec; integer_hash_spec; set_item_spec; get_item_spec]).
-
-Lemma body_surely_malloc: semax_body Vprog Gprog f_surely_malloc surely_malloc_spec.
-Proof.
-  start_function.
-  forward_call n.
-  Intros p.
-  forward_if
-  (PROP ( )
-   LOCAL (temp _p p)
-   SEP (malloc_token Tsh n p * memory_block Tsh n p)).
-  - if_tac; entailer!.
-  - forward_call tt.
-    contradiction.
-  - if_tac.
-    + forward. subst p. discriminate.
-    + Intros. forward. entailer!.
-  - forward. Exists p; entailer!.
-Qed.
+Definition Gprog : funspecs := ltac:(with_library prog [CAS_SC_spec; load_SC_spec; store_SC_spec;
+  integer_hash_spec; set_item_spec; get_item_spec]).
 
 Lemma body_integer_hash: semax_body Vprog Gprog f_integer_hash integer_hash_spec.
 Proof.
@@ -994,36 +153,21 @@ Ltac cancel_for_forward_call ::= repeat (rewrite ?sepcon_andp_prop', ?sepcon_and
 
 Ltac entailer_for_return ::= go_lower; entailer'.
 
-Lemma apply_int_ops : forall v h i (Hv : verif_atomics.apply_hist (Vint i) h = Some v)
-  (Hints : Forall int_op h), tc_val tint v.
-Proof.
-  induction h; simpl; intros.
-  - inv Hv; eauto.
-  - inversion Hints as [|?? Ha]; subst.
-    destruct a.
-    + destruct (eq_dec v0 (Vint i)); [eapply IHh; eauto | discriminate].
-    + destruct v0; try contradiction; eapply IHh; eauto.
-    + destruct (eq_dec r (Vint i)); [|discriminate].
-      destruct Ha as (? & ? & ?).
-      destruct w; try contradiction.
-      destruct (eq_dec c (Vint i)); eapply IHh; eauto.
-Qed.
-
 Lemma failed_CAS_fst : forall v h h', Forall2 (failed_CAS v) h h' -> map snd h' = map snd h.
 Proof.
   induction 1; auto.
   destruct H as (? & ? & ? & ? & ? & ? & ? & ?); simpl; f_equal; auto.
 Qed.
 
-Lemma indices_next : forall i j, ((j - i) mod 32) < 31 -> indices i (j + 1) = indices i j ++ [j mod 32].
+Lemma indices_next : forall i j, ((j - i) mod size) < size - 1 -> indices i (j + 1) = indices i j ++ [j mod size].
 Proof.
   intros; unfold indices.
-  exploit (Z_mod_lt (j - i) 32); [computable | intro].
+  exploit (Z_mod_lt (j - i) size); [apply size_pos | intro].
   rewrite Z.add_sub_swap, <- Zplus_mod_idemp_l, Zmod_small by omega.
   rewrite Z2Nat.inj_add by omega.
   rewrite upto_app, map_app; simpl.
   change (upto 1) with [0]; simpl.
-  rewrite Z2Nat.id, Z.add_0_r by omega.
+  rewrite Z2Nat.id, Z.add_0_r by (apply Z_mod_lt; computable).
   rewrite Zplus_mod_idemp_r, Zplus_minus; auto.
 Qed.
 
@@ -1032,52 +176,115 @@ Proof.
   start_function.
   forward_call key.
   eapply semax_pre with (P' := EX i : Z, EX i1 : Z, EX h' : list (hist * hist),
-    PROP (Zlength h' = Zlength h; i1 mod 32 = (i + hash key) mod 32; 0 <= i < 32;
+    PROP (Zlength h' = Zlength h; i1 mod size = (i + hash key) mod size; 0 <= i < size;
           forall j, (In j (indices (hash key) (i + hash key)) -> failed_CAS key (Znth j h ([], [])) (Znth j h' ([], []))) /\
             (~In j (indices (hash key) (i + hash key)) -> Znth j h' ([], []) = Znth j h ([], [])))
     LOCAL (temp _idx (vint i1); temp _key (vint key); temp _value (vint value); gvar _m_entries p)
-    SEP (data_at sh (tarray (tptr tentry) 32) entries p; fold_right sepcon emp (map (atomic_entry sh) entries);
-         entry_hists entries h')).
+    SEP (@data_at CompSpecs sh (tarray tentry size) entries p; atomic_entries sh entries h')).
   { Exists 0 (key * 654435761)%Z h; entailer!.
-    unfold hash at 1; rewrite Zmod_mod; split; auto.
+    rewrite Zmod_mod; split; auto.
     unfold indices; rewrite Zminus_diag; split; auto; contradiction. }
   eapply semax_loop.
   - Intros i i1 h'; forward.
     forward.
     rewrite sub_repr, and_repr; simpl.
-    rewrite Zland_two_p with (n := 5) by omega.
-    change (2 ^ 5) with 32.
-    exploit (Z_mod_lt i1 32); [omega | intro Hi1].
-    assert (0 <= i1 mod 32 < Zlength h') by omega.
-    assert_PROP (Zlength entries = 32) as Hentries by entailer!.
-    rewrite <- Hentries in Hi1 at 3.
-    assert (isptr (Znth (i1 mod 32) entries Vundef)).
-    { apply Forall_Znth; auto. }
-    forward.
-    forward.
+    rewrite Zland_two_p with (n := 14) by omega.
+    change (2 ^ 14) with size.
+    exploit (Z_mod_lt i1 size); [omega | intro Hi1].
+    assert (0 <= i1 mod size < Zlength h') by omega.
+    assert_PROP (Zlength entries = size) as Hentries by entailer!.
+    assert (0 <= i1 mod size < Zlength entries) by omega.
     assert (i <= Zlength h') by omega.
-    rewrite extract_nth_sepcon with (i := i1 mod 32), Znth_map with (d' := Vundef); try rewrite Zlength_map;
-      auto.
-    unfold entry_hists; erewrite extract_nth_sepcon with (i := i1 mod 32)(l := map _ _), Znth_map, Znth_upto; simpl;
-      auto; rewrite ?Zlength_map, ?Zlength_upto; simpl; try omega.
-    unfold atomic_entry; Intros lkey lval.
-    rewrite atomic_loc_isptr.
+    unfold atomic_entries; rewrite extract_nth_sepcon with (i := i1 mod size),
+      Znth_map with (d' := (Vundef, Vundef, ([], []))), Znth_combine
+      by (rewrite ?Zlength_map, ?Zlength_combine, ?Z.min_l; auto; omega).
+    destruct (Znth (i1 mod size) entries (Vundef, Vundef)) as (pki, pvi) eqn: Hpi.
+    destruct (Znth (i1 mod size) h' ([], [])) as (hki, hvi) eqn: Hhi.
+    unfold atomic_entry; Intros.
+    rewrite atomic_loc_isptr; Intros.
+
+Ltac solve_efield_denote Delta P Q R efs gfs H ::=   evar (gfs : list gfield);
+  assert (ENTAIL Delta, PROPx P (LOCALx Q (SEPx R)) |-- efield_denote efs gfs) as H; 
+  [
+    unfold efs, gfs;
+    match goal with
+    | efs := nil |- _ =>
+      instantiate (1 := nil);
+      apply prop_right, I
+    | efs := ?ef :: ?efs' |- _ =>
+      let efs0 := fresh "efs" in
+      let gfs0 := fresh "gfs" in
+      let H0 := fresh "H" in
+      pose efs' as efs0;
+      solve_efield_denote Delta P Q R efs0 gfs0 H0;
+      match goal with
+      | gfs0 := ?gfs0' |- _ =>
+        match ef with
+        | eArraySubsc ?ei => 
+
+          let HA := fresh "H" in
+          let vi := fresh "vi" in evar (vi: val);
+          do_compute_expr Delta P Q R ei vi HA;
+
+          revert vi HA;
+          let vvvv := fresh "vvvv" in
+          let HHHH := fresh "HHHH" in
+            match goal with
+            | |- let vi := ?V in _ => remember V as vvvv eqn:HHHH
+            end;
+          autorewrite with norm in HHHH;
+      
+          match type of HHHH with
+          | _ = Vint (Int.repr _) => idtac
+          | _ = Vint (Int.sub _ _) => unfold Int.sub in HHHH
+          | _ = Vint (Int.add _ _) => unfold Int.add in HHHH
+          | _ = Vint (Int.mul _ _) => unfold Int.mul in HHHH
+          | _ = Vint (Int.and _ _) => unfold Int.and in HHHH
+          | _ = Vint (Int.or _ _) => unfold Int.or in HHHH
+          | _ = Vint ?V =>
+            replace V with (Int.repr (Int.unsigned V)) in HHHH
+              by (rewrite (Int.repr_unsigned V); reflexivity)
+          end;
+          (* subst vvvv; *)
+          rewrite HHHH in *; clear HHHH; (* Without this replacement, subst fails, and the next forward runs forever! *)
+          intros vi HA;
+
+          match goal with
+          | vi := Vint (Int.repr ?i) |- _ => instantiate (1 := ArraySubsc i :: gfs0')
+          end;
+          
+          let HB := fresh "H" in
+          assert (match typeof ei with | Tint _ _ _ => True | _ => False end) as HB by (simpl; auto);
+          
+          apply (efield_denote_cons_array _ _ _ _ _ H0 HA HB)
+
+        | eStructField ?i =>
+          instantiate (1 := StructField i :: gfs0');
+          apply efield_denote_cons_struct, H0
+        | eUnionField ?i =>
+          instantiate (1 := UnionField i :: gfs0');
+          apply efield_denote_cons_union, H0
+        end
+      end
+    end
+  |].
+
     forward.
-    destruct (Znth (i1 mod 32) h' ([], [])) as (hki, hvi) eqn: Hhi.
-    assert (~ In (i1 mod 32) (indices (hash key) (i + hash key))) as Hnew.
+    { entailer!.
+      setoid_rewrite Hpi; auto. }
+    assert (~ In (i1 mod size) (indices (hash key) (i + hash key))) as Hnew.
     { unfold indices; rewrite in_map_iff; intros (? & Heq & Hin).
-      rewrite Z.add_simpl_r, In_upto, Z2Nat.id in Hin by (apply Z_mod_lt; computable).
-      replace (i1 mod 32) with ((i + hash key) mod 32) in Heq.
-      rewrite Z.add_comm in Heq; apply Zmod_plus_inv in Heq; [|computable].
+      rewrite Z.add_simpl_r, In_upto, Z2Nat.id in Hin by (apply Z_mod_lt, size_pos).
+      replace (i1 mod size) with ((i + hash key) mod size) in Heq.
+      rewrite Z.add_comm in Heq; apply Zmod_plus_inv in Heq; [|apply size_pos].
       rewrite Zmod_small in Heq; [omega|].
-      destruct Hin; split; auto; etransitivity; eauto; apply Z_mod_lt; computable. }
-    assert (Znth (i1 mod 32) h ([], []) = Znth (i1 mod 32) h' ([], [])) as Heq.
+      destruct Hin; split; auto; etransitivity; eauto; apply Z_mod_lt, size_pos. }
+    assert (Znth (i1 mod size) h ([], []) = Znth (i1 mod size) h' ([], [])) as Heq.
     { match goal with H : forall j, (In j _ -> _) /\ (~In j _ -> _) |- _ => symmetry; apply H; auto end. }
     assert (ordered_hist hki).
-    { match goal with H : wf_hists h |- _ => eapply Forall_Znth with (i0 := i1 mod 32) in H; [|omega];
+    { match goal with H : wf_hists h |- _ => eapply Forall_Znth with (i0 := i1 mod size) in H; [|omega];
       rewrite Heq, Hhi in H; tauto end. }
-    forward_call (Tsh, sh, field_address tentry [StructField _key] (Znth (i1 mod 32) entries Vundef), lkey, vint 0,
-      hki, fun (h : hist) => !!(h = hki) && emp, k_R,
+    forward_call (sh, pki, vint 0, hki, fun (h : hist) => !!(h = hki) && emp, k_R,
       fun (h : hist) (v : val) => !!(forall v0, last_value hki v0 -> v0 <> vint 0 -> v = v0) && emp).
     { entailer!.
       rewrite field_address_offset; simpl.
@@ -1107,7 +314,7 @@ Proof.
           hki' = hki ++ [(t, Load (vint 0)); (t', CAS (Vint r) (vint 0) (vint key))] /\
             (r = Int.zero \/ r = Int.repr key) /\
           forall v0 : val, last_value hki v0 -> v0 <> vint 0 -> Vint r = v0)
-      (LOCALx Q (SEPx (ghost_hist hki' (field_address tentry [StructField _key] (Znth (i1 mod 32) entries Vundef)) :: R))))
+      (LOCALx Q (SEPx (ghost_hist hki' (field_address tentry [StructField _key] (Znth (i1 mod size) entries Vundef)) :: R))))
     end.
     + match goal with |- semax _ (PROP () (LOCALx ?Q (SEPx ?R))) _ _ =>
         forward_if (PROP (i0 = Int.zero) (LOCALx Q (SEPx R))) end.
@@ -1116,13 +323,13 @@ Proof.
         destruct (eq_dec EK_continue EK_normal); [discriminate|].
         unfold loop1_ret_assert.
         instantiate (1 := EX i : Z, EX i1 : Z, EX h' : list (hist * hist),
-          PROP (Zlength h' = Zlength h; i1 mod 32 = (i + hash key) mod 32; 0 <= i < 32;
+          PROP (Zlength h' = Zlength h; i1 mod size = (i + hash key) mod size; 0 <= i < size;
           forall j, (In j (indices (hash key) ((i + 1) + hash key)) -> failed_CAS key (Znth j h ([], [])) (Znth j h' ([], []))) /\
             (~In j (indices (hash key) ((i + 1) + hash key)) -> Znth j h' ([], []) = Znth j h ([], [])))
           LOCAL (temp _idx (vint i1); temp _key (vint key); temp _value (vint value); gvar _m_entries p)
-          SEP (data_at sh (tarray (tptr tentry) 32) entries p; fold_right sepcon emp (map (atomic_entry sh) entries);
+          SEP (data_at sh (tarray (tptr tentry) size) entries p; fold_right sepcon emp (map (atomic_entry sh) entries);
                entry_hists entries h')).
-        Exists i (i1 mod 32) (upd_Znth (i1 mod 32) h' (fst (Znth (i1 mod 32) h' ([], [])) ++ [(t, Load (Vint i0))], snd (Znth (i1 mod 32) h' ([], [])))).
+        Exists i (i1 mod size) (upd_Znth (i1 mod size) h' (fst (Znth (i1 mod size) h' ([], [])) ++ [(t, Load (Vint i0))], snd (Znth (i1 mod size) h' ([], [])))).
         go_lower.
         apply andp_right.
         { apply prop_right; split.
@@ -1136,7 +343,7 @@ Proof.
               match goal with H : forall j, (In j _ -> _) /\ (~In j _ -> _) |- _ => apply H; auto end.
               { intro; contradiction Hnew; subst; auto. } }
             simpl in Hin; destruct Hin; [subst | contradiction].
-            replace ((i + hash key) mod 32) with (i1 mod 32).
+            replace ((i + hash key) mod size) with (i1 mod size).
             rewrite upd_Znth_same by auto.
             rewrite Heq, Hhi; repeat eexists; eauto; auto.
             match goal with H : forall v0, last_value hki v0 -> v0 <> vint 0 -> Vint i0 = v0 |- _ =>
@@ -1153,7 +360,7 @@ Proof.
         * rewrite replace_nth_sepcon; apply sepcon_list_derives.
           { rewrite upd_Znth_Zlength; rewrite !Zlength_map; auto. }
           rewrite upd_Znth_Zlength; rewrite !Zlength_map; auto; intros.
-          destruct (eq_dec i2 (i1 mod 32)).
+          destruct (eq_dec i2 (i1 mod size)).
           subst; rewrite upd_Znth_same by (rewrite Zlength_map; auto).
           rewrite Znth_map with (d' := Vundef) by auto.
           unfold atomic_entry.
@@ -1163,7 +370,7 @@ Proof.
           apply sepcon_list_derives.
           { rewrite upd_Znth_Zlength; rewrite !Zlength_map, Zlength_upto; auto; simpl; omega. }
           rewrite upd_Znth_Zlength; rewrite !Zlength_map; auto; intros.
-          destruct (eq_dec i2 (i1 mod 32)).
+          destruct (eq_dec i2 (i1 mod size)).
           subst; rewrite upd_Znth_same by (rewrite Zlength_map; auto).
           erewrite Znth_map, Znth_upto; simpl; auto; try omega.
           rewrite upd_Znth_same; auto; simpl.
@@ -1178,7 +385,7 @@ Proof.
       { forward.
         entailer!. }
       Intros; subst.
-      forward_call (Tsh, sh, field_address tentry [StructField _key] (Znth (i1 mod 32) entries Vundef), lkey, vint 0,
+      forward_call (Tsh, sh, field_address tentry [StructField _key] (Znth (i1 mod size) entries Vundef), lkey, vint 0,
         vint key, vint 0, hki ++ [(t, Load (vint 0))],
         fun (h : hist) c v => !!(c = vint 0 /\ v = vint key /\ h = hki ++ [(t, Load (vint 0))]) && emp,
         k_R, fun (h : hist) (v : val) => !!(forall v0, last_value hki v0 -> v0 <> vint 0 -> v = v0) && emp).
@@ -1230,8 +437,8 @@ Proof.
         destruct (eq_dec EK_continue EK_normal); [discriminate|].
         unfold loop1_ret_assert.
         go_lower.
-        Exists i (i1 mod 32) (upd_Znth (i1 mod 32) h' (fst (Znth (i1 mod 32) h' ([], [])) ++
-          [(t, Load (vint 0)); (t', CAS (Vint i0) (vint 0) (vint key))], snd (Znth (i1 mod 32) h' ([], [])))).
+        Exists i (i1 mod size) (upd_Znth (i1 mod size) h' (fst (Znth (i1 mod size) h' ([], [])) ++
+          [(t, Load (vint 0)); (t', CAS (Vint i0) (vint 0) (vint key))], snd (Znth (i1 mod size) h' ([], [])))).
         apply andp_right.
         { apply prop_right; split.
           { rewrite upd_Znth_Zlength; auto; omega. }
@@ -1244,7 +451,7 @@ Proof.
               match goal with H : forall j, (In j _ -> _) /\ (~In j _ -> _) |- _ => apply H; auto end.
               { intro; contradiction Hnew; subst; auto. } }
             simpl in Hin; destruct Hin; [subst | contradiction].
-            replace ((i + hash key) mod 32) with (i1 mod 32).
+            replace ((i + hash key) mod size) with (i1 mod size).
             rewrite upd_Znth_same by auto.
             match goal with H : Forall _ (hki ++ _) |- _ => rewrite Forall_app in H; destruct H as (? & Ht);
               inv Ht end.
@@ -1263,7 +470,7 @@ Proof.
         * rewrite replace_nth_sepcon; apply sepcon_list_derives.
           { rewrite upd_Znth_Zlength; rewrite !Zlength_map; auto. }
           rewrite upd_Znth_Zlength; rewrite !Zlength_map; auto; intros.
-          destruct (eq_dec i2 (i1 mod 32)).
+          destruct (eq_dec i2 (i1 mod size)).
           subst; rewrite upd_Znth_same by (rewrite Zlength_map; auto).
           rewrite Znth_map with (d' := Vundef) by auto.
           unfold atomic_entry.
@@ -1273,7 +480,7 @@ Proof.
           apply sepcon_list_derives.
           { rewrite upd_Znth_Zlength; rewrite !Zlength_map, Zlength_upto; auto; simpl; omega. }
           rewrite upd_Znth_Zlength; rewrite !Zlength_map; auto; intros.
-          destruct (eq_dec i2 (i1 mod 32)).
+          destruct (eq_dec i2 (i1 mod size)).
           subst; rewrite upd_Znth_same by (rewrite Zlength_map; auto).
           erewrite Znth_map, Znth_upto; simpl; auto; try omega.
           rewrite upd_Znth_same; auto; simpl.
@@ -1305,7 +512,7 @@ Proof.
       Intros hki'.
       forward.
       forward.
-      forward_call (Tsh, sh, field_address tentry [StructField _value] (Znth (i1 mod 32) entries Vundef), lval,
+      forward_call (Tsh, sh, field_address tentry [StructField _value] (Znth (i1 mod size) entries Vundef), lval,
         vint value, vint 0, hvi, fun (h : hist) v => !!(v = vint value) && emp, v_R, fun (h : hist) => emp).
       { entailer!.
         rewrite field_address_offset; auto.
@@ -1320,7 +527,7 @@ Proof.
         eapply derives_trans, precise_weak_precise; auto. }
       Intros t'.
       forward.
-      Exists (i1 mod 32) (upd_Znth (i1 mod 32) h' (hki', hvi ++ [(t', Store (vint value))])).
+      Exists (i1 mod size) (upd_Znth (i1 mod size) h' (hki', hvi ++ [(t', Store (vint value))])).
       apply andp_right; auto.
       apply andp_right.
       { apply prop_right; split; auto.
@@ -1344,9 +551,9 @@ Proof.
               match goal with H : forall v0, last_value hki v0 -> v0 <> vint 0 -> Vint x = v0 |- _ =>
                 symmetry; apply H; auto end.
               rewrite ordered_last_value; auto.
-        - assert (indices (hash key) (i + hash key) = indices (hash key) (i1 mod 32)) as Hindex.
+        - assert (indices (hash key) (i + hash key) = indices (hash key) (i1 mod size)) as Hindex.
           { unfold indices.
-            replace (i1 mod 32) with ((i + hash key) mod 32).
+            replace (i1 mod size) with ((i + hash key) mod size).
             rewrite Zminus_mod_idemp_l; auto. }
           split.
           + intro Hin.
@@ -1367,7 +574,7 @@ Proof.
       * rewrite replace_nth_sepcon; apply sepcon_list_derives.
         { rewrite upd_Znth_Zlength; rewrite !Zlength_map; auto. }
         rewrite upd_Znth_Zlength; rewrite !Zlength_map; auto; intros.
-        destruct (eq_dec i2 (i1 mod 32)).
+        destruct (eq_dec i2 (i1 mod size)).
         subst; rewrite upd_Znth_same by (rewrite Zlength_map; auto).
         rewrite Znth_map with (d' := Vundef) by auto.
         unfold atomic_entry.
@@ -1378,7 +585,7 @@ Proof.
         apply sepcon_list_derives.
         { rewrite upd_Znth_Zlength; rewrite !Zlength_map, Zlength_upto; simpl; omega. }
         rewrite upd_Znth_Zlength; rewrite !Zlength_map; auto; intros.
-        destruct (eq_dec i2 (i1 mod 32)).
+        destruct (eq_dec i2 (i1 mod size)).
         subst; rewrite upd_Znth_same by (rewrite Zlength_map; auto).
         erewrite Znth_map, Znth_upto; simpl; auto; try omega.
         rewrite upd_Znth_same; auto; simpl.
@@ -1394,7 +601,7 @@ Proof.
     Exists (i + 1) (i1 + 1) h'; entailer!.
     split.
     { rewrite <- Zplus_mod_idemp_l.
-      replace (i1 mod 32) with ((i + hash key) mod 32).
+      replace (i1 mod size) with ((i + hash key) mod size).
       rewrite Zplus_mod_idemp_l, <- Z.add_assoc, (Z.add_comm _ 1), Z.add_assoc; auto. }
     admit. (* list is long enough *)
 Admitted.
@@ -1410,51 +617,50 @@ Proof.
   start_function.
   forward_call key.
   eapply semax_pre with (P' := EX i : Z, EX i1 : Z, EX h' : list (hist * hist),
-    PROP (Zlength h' = Zlength h; i1 mod 32 = (i + hash key) mod 32; 0 <= i < 32;
+    PROP (Zlength h' = Zlength h; i1 mod size = (i + hash key) mod size; 0 <= i < size;
           forall j, (In j (indices (hash key) (i + hash key)) -> failed_load key (Znth j h ([], [])) (Znth j h' ([], []))) /\
             (~In j (indices (hash key) (i + hash key)) -> Znth j h' ([], []) = Znth j h ([], [])))
     LOCAL (temp _idx (vint i1); temp _key (vint key); gvar _m_entries p)
-    SEP (data_at sh (tarray (tptr tentry) 32) entries p; fold_right sepcon emp (map (atomic_entry sh) entries);
-         entry_hists entries h')).
+    SEP (data_at sh (tarray (tptr tentry) size) entries p; ; atomic_entries sh entries h')).
   { Exists 0 (key * 654435761)%Z h; entailer!.
-    unfold hash at 1; rewrite Zmod_mod; split; auto.
+    rewrite Zmod_mod; split; auto.
     unfold indices; rewrite Zminus_diag; split; auto; contradiction. }
   eapply semax_loop.
   - Intros i i1 h'; forward.
     forward.
     rewrite sub_repr, and_repr; simpl.
-    rewrite Zland_two_p with (n := 5) by omega.
-    change (2 ^ 5) with 32.
-    exploit (Z_mod_lt i1 32); [omega | intro Hi1].
-    assert (0 <= i1 mod 32 < Zlength h') by omega.
-    assert_PROP (Zlength entries = 32) as Hentries by entailer!.
+    rewrite Zland_two_p with (n := 14) by omega.
+    change (2 ^ 14) with size.
+    exploit (Z_mod_lt i1 size); [omega | intro Hi1].
+    assert (0 <= i1 mod size < Zlength h') by omega.
+    assert_PROP (Zlength entries = size) as Hentries by entailer!.
     rewrite <- Hentries in Hi1 at 3.
-    assert (isptr (Znth (i1 mod 32) entries Vundef)).
+    assert (isptr (Znth (i1 mod size) entries Vundef)).
     { apply Forall_Znth; auto. }
     forward.
     forward.
     assert (i <= Zlength h') by omega.
-    rewrite extract_nth_sepcon with (i := i1 mod 32), Znth_map with (d' := Vundef); try rewrite Zlength_map;
+    rewrite extract_nth_sepcon with (i := i1 mod size), Znth_map with (d' := Vundef); try rewrite Zlength_map;
       auto.
-    unfold entry_hists; erewrite extract_nth_sepcon with (i := i1 mod 32)(l := map _ _), Znth_map, Znth_upto; simpl;
+    unfold entry_hists; erewrite extract_nth_sepcon with (i := i1 mod size)(l := map _ _), Znth_map, Znth_upto; simpl;
       auto; rewrite ?Zlength_map, ?Zlength_upto; simpl; try omega.
     unfold atomic_entry; Intros lkey lval.
     rewrite atomic_loc_isptr.
     forward.
-    destruct (Znth (i1 mod 32) h' ([], [])) as (hki, hvi) eqn: Hhi.
-    assert (~ In (i1 mod 32) (indices (hash key) (i + hash key))) as Hnew.
+    destruct (Znth (i1 mod size) h' ([], [])) as (hki, hvi) eqn: Hhi.
+    assert (~ In (i1 mod size) (indices (hash key) (i + hash key))) as Hnew.
     { unfold indices; rewrite in_map_iff; intros (? & Heq & Hin).
       rewrite Z.add_simpl_r, In_upto, Z2Nat.id in Hin by (apply Z_mod_lt; computable).
-      replace (i1 mod 32) with ((i + hash key) mod 32) in Heq.
+      replace (i1 mod size) with ((i + hash key) mod size) in Heq.
       rewrite Z.add_comm in Heq; apply Zmod_plus_inv in Heq; [|computable].
       rewrite Zmod_small in Heq; [omega|].
       destruct Hin; split; auto; etransitivity; eauto; apply Z_mod_lt; computable. }
-    assert (Znth (i1 mod 32) h ([], []) = Znth (i1 mod 32) h' ([], [])) as Heq.
+    assert (Znth (i1 mod size) h ([], []) = Znth (i1 mod size) h' ([], [])) as Heq.
     { match goal with H : forall j, (In j _ -> _) /\ (~In j _ -> _) |- _ => symmetry; apply H; auto end. }
     assert (ordered_hist hki).
-    { match goal with H : wf_hists h |- _ => eapply Forall_Znth with (i0 := i1 mod 32) in H; [|omega];
+    { match goal with H : wf_hists h |- _ => eapply Forall_Znth with (i0 := i1 mod size) in H; [|omega];
       rewrite Heq, Hhi in H; tauto end. }
-    forward_call (Tsh, sh, field_address tentry [StructField _key] (Znth (i1 mod 32) entries Vundef), lkey, vint 0,
+    forward_call (Tsh, sh, field_address tentry [StructField _key] (Znth (i1 mod size) entries Vundef), lkey, vint 0,
       hki, fun h => !!(h = hki) && emp, k_R,
       fun (h : hist) (v : val) => !!(forall v0, last_value hki v0 -> v0 <> vint 0 -> v = v0) && emp).
     { entailer!.
@@ -1483,8 +689,8 @@ Proof.
     + rewrite (atomic_loc_isptr _ lval).
       forward.
       forward.
-      forward_call (Tsh, sh, field_address tentry [StructField _value] (Znth (i1 mod 32) entries Vundef), lval, vint 0,
-        snd (Znth (i1 mod 32) h' ([], [])), fun (h : hist) => emp, v_R, fun (h : hist) (v : val) => emp).
+      forward_call (Tsh, sh, field_address tentry [StructField _value] (Znth (i1 mod size) entries Vundef), lval, vint 0,
+        snd (Znth (i1 mod size) h' ([], [])), fun (h : hist) => emp, v_R, fun (h : hist) (v : val) => emp).
       { entailer!.
         rewrite field_address_offset; auto.
         { rewrite field_compatible_cons; simpl.
@@ -1499,8 +705,8 @@ Proof.
         eapply derives_trans, precise_weak_precise; auto. }
       Intros x; destruct x as (t', v); simpl in *.
       forward.
-      Exists (Int.signed v) (i1 mod 32) (upd_Znth (i1 mod 32) h' (fst (Znth (i1 mod 32) h' ([], [])) ++ [(t, Load (vint key))],
-        snd (Znth (i1 mod 32) h' ([], [])) ++ [(t', Load (Vint v))])).
+      Exists (Int.signed v) (i1 mod size) (upd_Znth (i1 mod size) h' (fst (Znth (i1 mod size) h' ([], [])) ++ [(t, Load (vint key))],
+        snd (Znth (i1 mod size) h' ([], [])) ++ [(t', Load (Vint v))])).
       apply andp_right.
       { apply prop_right.
         split; [apply Int.signed_range|].
@@ -1514,9 +720,9 @@ Proof.
             match goal with H : forall v0, last_value hki v0 -> v0 <> vint 0 -> vint key = v0 |- _ =>
               symmetry; apply H; auto end.
             rewrite ordered_last_value; auto.
-        - assert (indices (hash key) (i + hash key) = indices (hash key) (i1 mod 32)) as Hindex.
+        - assert (indices (hash key) (i + hash key) = indices (hash key) (i1 mod size)) as Hindex.
           { unfold indices.
-            replace (i1 mod 32) with ((i + hash key) mod 32).
+            replace (i1 mod size) with ((i + hash key) mod size).
             rewrite Zminus_mod_idemp_l; auto. }
           split.
           + intro Hin.
@@ -1537,7 +743,7 @@ Proof.
       * rewrite replace_nth_sepcon; apply sepcon_list_derives.
         { rewrite upd_Znth_Zlength; rewrite !Zlength_map; auto. }
         rewrite upd_Znth_Zlength; rewrite !Zlength_map; auto; intros.
-        destruct (eq_dec i0 (i1 mod 32)).
+        destruct (eq_dec i0 (i1 mod size)).
         subst; rewrite upd_Znth_same by (rewrite Zlength_map; auto).
         rewrite Znth_map with (d' := Vundef) by auto.
         unfold atomic_entry.
@@ -1547,7 +753,7 @@ Proof.
         rewrite Hhi; apply sepcon_list_derives.
         { rewrite upd_Znth_Zlength; rewrite !Zlength_map, Zlength_upto; simpl; omega. }
         rewrite upd_Znth_Zlength; rewrite !Zlength_map; auto; intros.
-        destruct (eq_dec i0 (i1 mod 32)).
+        destruct (eq_dec i0 (i1 mod size)).
         subst; rewrite upd_Znth_same by (rewrite Zlength_map; auto).
         erewrite Znth_map, Znth_upto; simpl; auto; try omega.
         rewrite upd_Znth_same; auto; simpl.
@@ -1562,7 +768,7 @@ Proof.
     + Intros; match goal with |- semax _ (PROP () (LOCALx ?Q (SEPx ?R))) _ _ =>
         forward_if (PROP (i0 <> Int.zero) (LOCALx Q (SEPx R))) end.
       * forward.
-        Exists 0 (i1 mod 32) (upd_Znth (i1 mod 32) h' (fst (Znth (i1 mod 32) h' ([], [])) ++ [(t, Load (vint 0))], snd (Znth (i1 mod 32) h' ([], [])))).
+        Exists 0 (i1 mod size) (upd_Znth (i1 mod size) h' (fst (Znth (i1 mod size) h' ([], [])) ++ [(t, Load (vint 0))], snd (Znth (i1 mod size) h' ([], [])))).
         apply andp_right.
         { apply prop_right.
           split; [split; computable|].
@@ -1576,9 +782,9 @@ Proof.
           match goal with H : forall v0, last_value hki v0 -> v0 <> vint 0 -> vint 0 = v0 |- _ =>
             symmetry; apply H; auto end.
           rewrite ordered_last_value; auto.
-        - assert (indices (hash key) (i + hash key) = indices (hash key) (i1 mod 32)) as Hindex.
+        - assert (indices (hash key) (i + hash key) = indices (hash key) (i1 mod size)) as Hindex.
           { unfold indices.
-            replace (i1 mod 32) with ((i + hash key) mod 32).
+            replace (i1 mod size) with ((i + hash key) mod size).
             rewrite Zminus_mod_idemp_l; auto. }
           split.
           + intro Hin.
@@ -1599,7 +805,7 @@ Proof.
         -- rewrite replace_nth_sepcon; apply sepcon_list_derives.
            { rewrite upd_Znth_Zlength; rewrite !Zlength_map; auto. }
            rewrite upd_Znth_Zlength; rewrite !Zlength_map; auto; intros.
-           destruct (eq_dec i0 (i1 mod 32)).
+           destruct (eq_dec i0 (i1 mod size)).
            subst; rewrite upd_Znth_same by (rewrite Zlength_map; auto).
            rewrite Znth_map with (d' := Vundef) by auto.
            unfold atomic_entry.
@@ -1609,7 +815,7 @@ Proof.
            rewrite Hhi; apply sepcon_list_derives.
            { rewrite upd_Znth_Zlength; rewrite !Zlength_map, Zlength_upto; simpl; omega. }
            rewrite upd_Znth_Zlength; rewrite !Zlength_map; auto; intros.
-           destruct (eq_dec i0 (i1 mod 32)).
+           destruct (eq_dec i0 (i1 mod size)).
            subst; rewrite upd_Znth_same by (rewrite Zlength_map; auto).
            erewrite Znth_map, Znth_upto; simpl; auto; try omega.
            rewrite upd_Znth_same; auto; simpl.
@@ -1627,13 +833,13 @@ Proof.
         destruct (eq_dec ek EK_normal); [subst | apply drop_tc_environ].
         Intros; unfold POSTCONDITION, abbreviate, normal_ret_assert, loop1_ret_assert.
         instantiate (1 := EX i : Z, EX i1 : Z, EX h' : list (hist * hist),
-          PROP (Zlength h' = Zlength h; i1 mod 32 = (i + hash key) mod 32; 0 <= i < 32;
+          PROP (Zlength h' = Zlength h; i1 mod size = (i + hash key) mod size; 0 <= i < size;
           forall j, (In j (indices (hash key) ((i + 1) + hash key)) -> failed_load key (Znth j h ([], [])) (Znth j h' ([], []))) /\
             (~In j (indices (hash key) ((i + 1) + hash key)) -> Znth j h' ([], []) = Znth j h ([], [])))
           LOCAL (temp _idx (vint i1); temp _key (vint key); gvar _m_entries p)
-          SEP (data_at sh (tarray (tptr tentry) 32) entries p; fold_right sepcon emp (map (atomic_entry sh) entries);
+          SEP (data_at sh (tarray (tptr tentry) size) entries p; fold_right sepcon emp (map (atomic_entry sh) entries);
                entry_hists entries h')).
-        Exists i (i1 mod 32) (upd_Znth (i1 mod 32) h' (fst (Znth (i1 mod 32) h' ([], [])) ++ [(t, Load (Vint i0))], snd (Znth (i1 mod 32) h' ([], [])))).
+        Exists i (i1 mod size) (upd_Znth (i1 mod size) h' (fst (Znth (i1 mod size) h' ([], [])) ++ [(t, Load (Vint i0))], snd (Znth (i1 mod size) h' ([], [])))).
         go_lower.
         apply andp_right.
         { apply prop_right; split.
@@ -1647,7 +853,7 @@ Proof.
               match goal with H : forall j, (In j _ -> _) /\ (~In j _ -> _) |- _ => apply H; auto end.
               { intro; contradiction Hnew; subst; auto. } }
             simpl in Hin; destruct Hin; [subst | contradiction].
-            replace ((i + hash key) mod 32) with (i1 mod 32).
+            replace ((i + hash key) mod size) with (i1 mod size).
             rewrite upd_Znth_same by auto.
             rewrite Heq, Hhi; repeat eexists; eauto; auto.
             match goal with H : forall v0, last_value hki v0 -> v0 <> vint 0 -> Vint i0 = v0 |- _ =>
@@ -1664,7 +870,7 @@ Proof.
         -- rewrite replace_nth_sepcon; apply sepcon_list_derives.
            { rewrite upd_Znth_Zlength; rewrite !Zlength_map; auto. }
            rewrite upd_Znth_Zlength; rewrite !Zlength_map; auto; intros.
-           destruct (eq_dec i2 (i1 mod 32)).
+           destruct (eq_dec i2 (i1 mod size)).
            subst; rewrite upd_Znth_same by (rewrite Zlength_map; auto).
            rewrite Znth_map with (d' := Vundef) by auto.
            unfold atomic_entry.
@@ -1674,7 +880,7 @@ Proof.
            rewrite Hhi; apply sepcon_list_derives.
            { rewrite upd_Znth_Zlength; rewrite !Zlength_map, Zlength_upto; simpl; omega. }
            rewrite upd_Znth_Zlength; rewrite !Zlength_map; auto; intros.
-           destruct (eq_dec i2 (i1 mod 32)).
+           destruct (eq_dec i2 (i1 mod size)).
            subst; rewrite upd_Znth_same by (rewrite Zlength_map; auto).
            erewrite Znth_map, Znth_upto; simpl; auto; try omega.
            rewrite upd_Znth_same; auto; simpl.
@@ -1691,7 +897,264 @@ Proof.
     Exists (i + 1) (i1 + 1) h'; entailer!.
     split.
     { rewrite <- Zplus_mod_idemp_l.
-      replace (i1 mod 32) with ((i + hash key) mod 32).
+      replace (i1 mod size) with ((i + hash key) mod size).
       rewrite Zplus_mod_idemp_l, <- Z.add_assoc, (Z.add_comm _ 1), Z.add_assoc; auto. }
     admit. (* list is long enough *)
 Admitted.
+
+(* Given the relations on histories, what can we actually conclude about the maps? *)
+Lemma make_map_eq : forall h h', Forall2 (fun a b => value_of_hist (fst a) = value_of_hist (fst b) /\
+  value_of_hist (snd a) = value_of_hist (snd b)) h h' -> make_map h = make_map h'.
+Proof.
+  induction 1; auto; simpl.
+  destruct x, y; simpl in *.
+  destruct H as (-> & ->); rewrite IHForall2; auto.
+Qed.
+
+Lemma make_map_no_key : forall h k (Hout : Forall (fun x => make_int (value_of_hist (fst x)) <> k) h),
+  Forall (fun x => fst x <> k) (make_map h).
+Proof.
+  induction h; simpl; auto; intros.
+  destruct a.
+  inv Hout.
+  constructor; auto.
+Qed.
+
+(* It would be nice if we could maintain the invariant that the map has no duplicates and is well-chained,
+   and indeed, the algorithm should maintain these properties. However, the per-slot histories do not obviously
+   present a way to prove this: if a new key has "mysteriously appeared" (i.e., been added by another thread),
+   we don't have a good way of knowing that it's well-chained. *)
+(* We can, however, allow for the possibility that there is garbage in the map, and consider the abstract map
+   to be those elements that can be successfully looked up, rather than all pairs in the map. In practice, this
+   *should* come down to the same thing, but how could we prove it? *)
+Lemma set_item_trace_map : forall h k v i h' (Hwf : wf_hists h) (Hlenh : Zlength h = size)
+  (Htrace : set_item_trace h k v i h') (Hk : k <> 0) (Hrepk : repable_signed k) (Hrepv : repable_signed v),
+  wf_hists h' /\ let m' := make_map (upd_Znth i h' (Znth i h ([], []))) in
+    map_incl (make_map h) m' /\ set m' k v = Some (make_map h').
+Proof.
+  intros.
+  destruct Htrace as (Hlen & Hbounds & Hi & Hrest).
+  destruct (Znth i h ([], [])) as (hk, hv) eqn: Hhi.
+  destruct Hi as (t & r & tv & Ht & Htv & Hi1 & Hi2 & Hr0).
+  assert (i <= Zlength h') by (rewrite Hlen; destruct Hbounds; apply Z.lt_le_incl; auto).
+  assert (0 <= i + 1 <= Zlength h').
+  { rewrite Hlen; destruct Hbounds; split; [|rewrite <- lt_le_1]; auto; omega. }
+  assert (vint k <> vint 0).
+  { intro; contradiction Hk; apply repr_inj_signed; auto.
+    { split; computable. }
+    { congruence. }}
+  assert (r = vint 0 \/ r = vint k) as Hr.
+  { destruct Hi1 as [(? & ?) | (? & ? & ? & ?)]; auto. }
+  assert ((if eq_dec r (vint 0) then vint k else r) = vint k) as Hif.
+  { if_tac; auto.
+    destruct Hr; [absurd (r = vint 0)|]; auto. }
+  assert (value_of_hist (fst (Znth i h' ([], []))) = vint k) as Hk'.
+  { destruct Hi1 as [(-> & ?) | (? & ? & -> & ?)].
+    - rewrite value_of_hist_snoc; auto.
+    - rewrite app_cons_assoc, value_of_hist_snoc; auto. }
+  assert (wf_hists h') as Hwf'; [|split; auto; split].
+  - unfold wf_hists; rewrite Forall_forall_Znth; intros j ?.
+    apply (Forall_Znth _ _ j ([], [])) in Hwf; [destruct Hwf as ((? & ?) & ? & ?) | omega].
+    destruct (eq_dec j i); [|specialize (Hrest j); destruct (in_dec Z_eq_dec j (indices (hash k) i))].
+    + subst; rewrite Hhi in *.
+      split; [|rewrite Hi2, map_app, Forall_app; repeat constructor; auto; apply ordered_snoc; auto].
+      destruct Hi1 as [(-> & _) | (? & ? & -> & _)]; rewrite map_app, Forall_app; repeat constructor;
+        auto; try (apply ordered_snoc; auto).
+      * rewrite app_cons_assoc; apply ordered_snoc; [apply ordered_snoc; auto|].
+        apply newer_snoc; auto.
+      * destruct Hr; subst; simpl; auto.
+    + destruct Hrest as ((? & ? & ? & Hcase & ? & ? & -> & ?) & _); auto; simpl in *.
+      split; auto.
+      destruct Hcase as [-> | (? & ? & ->)]; rewrite map_app, Forall_app; repeat constructor; auto.
+      * apply ordered_snoc; auto.
+      * rewrite app_cons_assoc; apply ordered_snoc; [apply ordered_snoc; auto|].
+        apply newer_snoc; auto.
+    + destruct Hrest as (_ & ->); auto.
+  - intros k0 v0 j Hk0 Hj.
+    exploit (Znth_inbounds j (make_map h) (0, 0)).
+    { rewrite Hj; intro X; inv X; contradiction Hk0; auto. }
+    intro; unfold make_map in *; rewrite <- upd_Znth_map.
+    rewrite Zlength_map in *.
+    rewrite Znth_map with (d' := ([], [])) in Hj by auto; inv Hj.
+    destruct (eq_dec j i); [subst; rewrite upd_Znth_same, Hhi; auto | rewrite upd_Znth_diff'];
+      rewrite ?Zlength_map in *; auto; try omega.
+    rewrite Znth_map with (d' := ([], [])) by omega.
+    specialize (Hrest j); destruct (in_dec Z_eq_dec j (indices (hash k) i));
+      [|destruct Hrest as (_ & ->); auto].
+    destruct Hrest as ((? & r1 & ? & Hcase & ? & ? & -> & Heq) & _); auto; simpl in *.
+    assert (value_of_hist (fst (Znth j h ([], []))) <> vint 0).
+    { intro X; rewrite X in Hk0; contradiction Hk0; auto. }
+    destruct Hcase as [-> | (? & ? & ->)].
+    + rewrite value_of_hist_snoc, Heq; auto.
+    + rewrite app_cons_assoc, value_of_hist_snoc, Heq; auto; simpl.
+      destruct (eq_dec (Vint r1) (vint 0)); auto.
+      absurd (r1 = Int.zero); auto; inv e; auto.
+  - assert (0 <= i < Zlength h') by (rewrite Hlen; auto).
+    unfold set.
+    assert (lookup (make_map (upd_Znth i h' (hk, hv))) k = Some i) as ->.
+    + unfold lookup, make_map.
+      assert (i = ((i - hash k) mod size + hash k) mod size) as Hmod.
+      { rewrite Zplus_mod_idemp_l, Z.sub_simpl_r, Zmod_small by omega; auto. }
+      pose proof (hash_range k).
+      assert (Zlength (map (fun hs => (make_int (value_of_hist (fst hs)), make_int (value_of_hist (snd hs))))
+              (upd_Znth i h' (hk, hv))) = size) as Hlen1.
+      { rewrite Zlength_map, upd_Znth_Zlength; auto; omega. }
+      erewrite index_of'_succeeds; simpl.
+      f_equal; symmetry; apply Hmod.
+      { rewrite Zlength_rebase; rewrite ?Zlength_map, ?upd_Znth_Zlength; auto; try omega.
+        replace (Zlength h') with size; [apply Z_mod_lt; computable | omega]. }
+      { rewrite Forall_forall; intros x Hin.
+        apply In_Znth with (d := (0, 0)) in Hin; destruct Hin as (j & Hj & Hx).
+        exploit (Z_mod_lt (i - hash k) size); [computable | intro].
+        rewrite Zlength_sublist in Hj; rewrite ?Zlength_rebase; rewrite ?Hlen1; try omega.
+        rewrite Znth_sublist, Z.add_0_r in Hx by (auto; omega).
+        rewrite Znth_rebase in Hx by omega.
+        rewrite Hlen1, Znth_map with (d' := ([], [])) in Hx.
+        subst x; simpl.
+        specialize (Hrest ((j + hash k) mod size)); destruct Hrest as ((? & r1 & ? & Hcase & ? & ? & ?) & _).
+        { unfold indices; rewrite in_map_iff.
+          exists j; split; [rewrite Z.add_comm; auto|].
+          rewrite In_upto, Z2Nat.id; omega. }
+        rewrite upd_Znth_diff'; auto.
+        destruct Hcase as [-> | (? & ? & ->)]; [|rewrite app_cons_assoc]; rewrite value_of_hist_snoc; simpl.
+        * split; intro X; [absurd (r1 = Int.zero) | absurd (r1 = Int.repr k)]; auto; apply signed_inj; auto.
+          rewrite Int.signed_repr; auto.
+        * destruct (eq_dec (Vint r1) (vint 0)); [absurd (r1 = Int.zero); auto; inversion e; auto | simpl].
+          split; intro X; [absurd (r1 = Int.zero) | absurd (r1 = Int.repr k)]; auto; apply signed_inj; auto.
+          rewrite Int.signed_repr; auto.
+        * intro X; rewrite <- X, Zminus_mod_idemp_l, Z.add_simpl_r, Z.sub_0_r, Zmod_small in Hj; try omega.
+          destruct Hj; split; auto; etransitivity; eauto; apply Z_mod_lt; computable.
+        * rewrite upd_Znth_Zlength by auto.
+          replace (Zlength h') with size by omega; apply Z_mod_lt; computable. }
+      { rewrite <- Hlen1, Znth_rebase', Znth_map with (d' := ([], [])); simpl;
+          rewrite ?Zlength_map, ?upd_Znth_Zlength; auto; try omega.
+        rewrite upd_Znth_same by auto; simpl.
+        destruct (eq_dec (value_of_hist hk) (vint 0)); [rewrite e; auto|].
+        rewrite Hr0; auto; destruct Hr; subst r; auto; simpl.
+        rewrite Int.signed_repr; auto. }
+    + simpl; unfold make_map; erewrite <- upd_Znth_map, upd_Znth_twice, upd_Znth_triv; rewrite ?Zlength_map;
+        auto.
+      rewrite Znth_map', Hk', Hi2, value_of_hist_snoc; simpl.
+      rewrite !Int.signed_repr; auto.
+Qed.
+
+Lemma get_item_trace_map : forall h k v i h' (Hwf : wf_hists h) (Hlenh : Zlength h = size)
+  (Htrace : get_item_trace h k v i h') (Hk : k <> 0) (Hrepk : repable_signed k) (Hrepv : repable_signed v),
+  wf_hists h' /\ match get (make_map h') k with
+  | Some v' => v' = v /\ map_incl (upd_Znth i (make_map h) (k, v)) (make_map h')
+  | None => v = 0 /\ map_incl (make_map h) (make_map h') end.
+Proof.
+  intros.
+  destruct Htrace as (Hlen & Hbounds & Hi & Hrest).
+  destruct (Znth i h ([], [])) as (hk, hv) eqn: Hhi.
+  destruct Hi as (t & r & Ht & Hi1 & Hi2 & Hr0).
+  assert (i <= Zlength h') by (rewrite Hlen; destruct Hbounds; apply Z.lt_le_incl; auto).
+  assert (0 <= i + 1 <= Zlength h').
+  { rewrite Hlen; destruct Hbounds; split; [|rewrite <- lt_le_1]; auto; omega. }
+  assert (vint k <> vint 0).
+  { intro; contradiction Hk; apply repr_inj_signed; auto.
+    { split; computable. }
+    { congruence. }}
+  assert (wf_hists h') as Hwf'; [|split; auto].
+  - unfold wf_hists; rewrite Forall_forall_Znth; intros j ?.
+    apply (Forall_Znth _ _ j ([], [])) in Hwf; [destruct Hwf as ((? & ?) & ? & ?) | omega].
+    destruct (eq_dec j i); [|specialize (Hrest j); destruct (in_dec Z_eq_dec j (indices (hash k) i))].
+    + subst; rewrite Hhi in *.
+      split; [rewrite Hi1, map_app, Forall_app; repeat constructor; auto; apply ordered_snoc; auto|].
+      destruct Hi2 as [(? & ? & ->) | (? & ? & ? & ->)]; auto.
+      rewrite map_app, Forall_app; repeat constructor; auto; apply ordered_snoc; auto.
+    + destruct Hrest as ((? & ? & ? & -> & ? & ? & -> & ?) & _); auto; simpl in *.
+      split; auto.
+      rewrite map_app, Forall_app; repeat constructor; auto.
+      apply ordered_snoc; auto.
+    + destruct Hrest as (_ & ->); auto.
+  - unfold get, lookup.
+    pose proof (index_of'_spec k (rebase (make_map h') (hash k))) as Hspec.
+    destruct (index_of' (rebase (make_map h') (hash k)) k) eqn: Hindex; simpl.
+    unfold make_map at 1; rewrite Znth_map with (d' := ([], [])).
+    pose proof (hash_range k).
+    assert ((z + hash k) mod size = i) as Hz.
+    { destruct Hspec as (Hz & Hcase & Hall).
+      assert (Zlength (make_map h') = Zlength h') as Hlenm by (unfold make_map; rewrite Zlength_map; auto).
+      assert (z <= (i - hash k) mod Zlength (make_map h')) as Hle.
+      { eapply Forall_sublist_le; try apply Hall; simpl.
+        { apply Z_mod_lt; omega. }
+        { omega. }
+        rewrite Znth_rebase' by omega.
+        unfold make_map; rewrite Znth_map'.
+        rewrite Hi1, value_of_hist_snoc; simpl.
+        destruct Hi2 as [(? & ? & ?) | (? & ?)]; subst; [|rewrite Int.signed_repr by auto]; tauto. }
+      rewrite Zlength_rebase in Hz by omega.
+      rewrite Znth_rebase, Hlenm in Hcase by omega.
+      unfold make_map in Hcase; rewrite Znth_map with (d' := ([], [])) in Hcase; simpl in Hcase.
+      destruct (eq_dec ((z + hash k) mod size) i); auto.
+      specialize (Hrest ((z + hash k) mod size)); destruct Hrest as ((? & r1 & ? & Hfst & ? & ? & ?) & _).
+      { unfold indices.
+        rewrite in_map_iff.
+        exists z; split; [rewrite Z.add_comm; auto|].
+        rewrite In_upto, Z2Nat.id.
+        rewrite Hlenm in Hle; replace (Zlength h') with size in Hle by omega.
+        destruct (eq_dec z ((i - hash k) mod size)); [|omega].
+        contradiction n; rewrite e, Zplus_mod_idemp_l, Z.sub_simpl_r, Zmod_small; auto; omega.
+        { apply Z_mod_lt; computable. } }
+      replace (Zlength h') with size in Hcase by omega.
+      rewrite Hfst, value_of_hist_snoc in Hcase; simpl in Hcase.
+      destruct Hcase; [absurd (r1 = Int.repr k) | absurd (r1 = Int.zero)]; auto; apply signed_inj; auto.
+      rewrite Int.signed_repr; auto.
+      { apply Z_mod_lt; omega. } }
+    rewrite Hz, Hi1.
+    replace (value_of_hist (hk ++ _)) with (vint r) by (rewrite value_of_hist_snoc; auto); simpl.
+    destruct Hi2 as [(? & ? & Hi2) | (? & ? & ? & Hi2)]; rewrite Hi2; clear dependent z; subst; simpl.
+    + split; auto.
+      intros k0 v0 j Hk0 Hj.
+      exploit (Znth_inbounds j (make_map h) (0, 0)).
+      { rewrite Hj; intro X; inv X; contradiction Hk0; auto. }
+      unfold make_map in *; rewrite Zlength_map; intro;
+        rewrite Znth_map with (d' := ([], [])) in Hj by auto; inv Hj.
+      rewrite Znth_map with (d' := ([], [])) by omega.
+      destruct (eq_dec j i).
+      { subst; rewrite Hhi in *; simpl in *; contradiction Hk0.
+        destruct (eq_dec (value_of_hist hk) (vint 0)); [rewrite e; auto|].
+        rewrite Hr0; auto. }
+      specialize (Hrest j); destruct (in_dec Z_eq_dec j (indices (hash k) i)).
+      * destruct Hrest as ((? & ? & ? & -> & ? & ? & -> & Heq) & _); auto.
+        rewrite value_of_hist_snoc; simpl.
+        destruct (eq_dec (value_of_hist (fst (Znth j h ([], [])))) (vint 0));
+          [contradiction Hk0; rewrite e; auto|].
+        rewrite Heq; auto.
+      * destruct Hrest as (_ & ->); auto.
+    + rewrite value_of_hist_snoc; simpl.
+      rewrite !Int.signed_repr by auto.
+      if_tac; [contradiction Hk; auto|].
+      split; auto.
+      intros k0 v0 j Hk0 Hj.
+      exploit (Znth_inbounds j (upd_Znth i (make_map h) (k, v)) (0, 0)).
+      { rewrite Hj; intro X; inv X; contradiction Hk0; auto. }
+      unfold make_map in *; rewrite upd_Znth_Zlength; rewrite Zlength_map; auto.
+      intro; rewrite Znth_map with (d' := ([], [])) by omega.
+      destruct (eq_dec j i).
+      { subst; rewrite upd_Znth_same in Hj by (rewrite Zlength_map; auto).
+        inv Hj; rewrite Hi1, Hi2.
+        rewrite !value_of_hist_snoc; simpl.
+        rewrite !Int.signed_repr; auto. }
+      rewrite upd_Znth_diff' in Hj; rewrite ?Zlength_map; auto.
+      rewrite Znth_map with (d' := ([], [])) in Hj by auto; inv Hj.
+      specialize (Hrest j); destruct (in_dec Z_eq_dec j (indices (hash k) i)).
+      * destruct Hrest as ((? & ? & ? & -> & ? & ? & -> & Heq) & _); auto.
+        rewrite value_of_hist_snoc; simpl.
+        destruct (eq_dec (value_of_hist (fst (Znth j h ([], [])))) (vint 0));
+          [contradiction Hk0; rewrite e; auto|].
+        rewrite Heq; auto.
+      * destruct Hrest as (_ & ->); auto.
+    + replace (Zlength h') with size by omega; apply Z_mod_lt; computable.
+    + assert (In r (map fst (rebase (make_map h') (hash k)))).
+      { rewrite in_map_iff.
+        unfold rebase, make_map; eexists; rewrite rotate_In, in_map_iff.
+        split; [|do 2 eexists; eauto; apply Znth_In with (i0 := i); omega].
+        rewrite Hi1, value_of_hist_snoc; simpl.
+        apply Int.signed_repr; destruct Hi2 as [(? & ? & ?) | (? & ?)]; subst; auto.
+        { pose proof (hash_range k).
+          rewrite Zlength_map; omega. } }
+      destruct Hspec as (Hnk & Hnz), Hi2 as [(? & ? & ?) | (? & ?)]; subst;
+        [contradiction Hnz | contradiction Hnk].
+Qed.
